src/Implementations/LogCache/FinishedNotCrashed.v
@@ -1,0 +1,1248 @@
+Require Import Lia Datatypes PeanoNat Compare_dec Framework TotalMem FSParameters Log Log.Specs.
+Require Import DiskLayer CryptoDiskLayer CacheLayer CachedDiskLayer. 
+Require Import Log LogCache LogCache.RepImplications.
+Require Import FunctionalExtensionality.
+
+
+
+Lemma BatchOperations_encrypt_all_finished_oracle_eq:
+forall u l1 l2 o1 o2 o3 o4 s1 s2 s1' s2' r1 r2 k1 k2,
+exec CryptoDiskLang u o1 s1
+(BatchOperations.encrypt_all k1 l1)  (Finished s1' r1) ->
+exec CryptoDiskLang u o2 s2
+(BatchOperations.encrypt_all k2 l2) (Finished s2' r2) ->
+o1 ++ o3 = o2 ++ o4 ->
+length l1 = length l2 ->
+o1 = o2.
+Proof.
+  induction l1; destruct l2; simpl; intros; try lia.
+  repeat invert_exec; eauto.
+  repeat invert_exec; cleanup; eauto.
+  repeat rewrite <- app_assoc in *; cleanup.
+  eapply IHl1 in H1; eauto.
+  subst; eauto.
+Qed.
+
+Lemma BatchOperations_hash_all_finished_oracle_eq:
+forall u l1 l2 o1 o2 o3 o4 s1 s2 s1' s2' r1 r2 k1 k2,
+exec CryptoDiskLang u o1 s1
+(BatchOperations.hash_all k1 l1)  (Finished s1' r1) ->
+exec CryptoDiskLang u o2 s2
+(BatchOperations.hash_all k2 l2) (Finished s2' r2) ->
+o1 ++ o3 = o2 ++ o4 ->
+length l1 = length l2 ->
+o1 = o2.
+Proof.
+  induction l1; destruct l2; simpl; intros; try lia.
+  repeat invert_exec; eauto.
+  repeat invert_exec; cleanup; eauto.
+  repeat rewrite <- app_assoc in *; cleanup.
+  eapply IHl1 in H1; eauto.
+  subst; eauto.
+Qed.
+
+Lemma BatchOperations_write_batch_finished_oracle_eq:
+forall u k1 k2 l1 l2 o1 o2 o3 o4 s1 s2 s1' s2' r1 r2 ,
+
+exec CryptoDiskLang u o1 s1
+(BatchOperations.write_batch k1 l1)  (Finished s1' r1) ->
+exec CryptoDiskLang u o2 s2
+(BatchOperations.write_batch k2 l2) (Finished s2' r2) ->
+o1 ++ o3 = o2 ++ o4 ->
+length k1 = length k2 ->
+length l1 = length l2 ->
+o1 = o2.
+Proof.
+  unfold BatchOperations.write_batch.
+  induction k1; destruct k2; simpl; intros; try lia.
+  repeat invert_exec; eauto.
+  repeat invert_exec; cleanup; eauto; simpl in *; try lia.
+  - repeat invert_exec; cleanup; eauto; try lia.
+  - repeat invert_exec; cleanup; eauto; try lia.
+  repeat rewrite <- app_assoc in *; cleanup.
+  eapply IHk1 in H1; eauto.
+  subst; eauto.
+Qed.
+
+Lemma BatchOperations_write_consecutive_finished_oracle_eq:
+forall u l1 l2 o1 o2 o3 o4 s1 s2 s1' s2' r1 r2 k1 k2,
+
+exec CryptoDiskLang u o1 s1
+(BatchOperations.write_consecutive k1 l1)  (Finished s1' r1) ->
+exec CryptoDiskLang u o2 s2
+(BatchOperations.write_consecutive k2 l2) (Finished s2' r2) ->
+o1 ++ o3 = o2 ++ o4 ->
+length l1 = length l2 ->
+o1 = o2.
+Proof.
+  unfold BatchOperations.write_consecutive.
+  induction l1; destruct l2; simpl; intros; try lia.
+  repeat invert_exec; eauto.
+  repeat invert_exec; cleanup; eauto.
+  repeat rewrite <- app_assoc in *; cleanup.
+  eapply IHl1 in H1; eauto.
+  subst; eauto.
+Qed.
+
+
+Lemma BatchOperations_read_consecutive_finished_oracle_eq:
+forall u l1 l2 o1 o2 o3 o4 s1 s2 s1' s2' r1 r2 k1 k2,
+exec CryptoDiskLang u o1 s1
+(BatchOperations.read_consecutive k1 l1)  (Finished s1' r1) ->
+exec CryptoDiskLang u o2 s2
+(BatchOperations.read_consecutive k2 l2) (Finished s2' r2) ->
+o1 ++ o3 = o2 ++ o4 ->
+l1 = l2 ->
+o1 = o2.
+Proof.
+  unfold BatchOperations.write_consecutive.
+  induction l1; simpl; intros; cleanup; try lia.
+  simpl in *; repeat invert_exec; eauto.
+  simpl in *; repeat invert_exec; cleanup; eauto.
+  repeat rewrite <- app_assoc in *; cleanup.
+  eapply IHl1 in H; eauto.
+  subst; eauto.
+Qed.
+
+Lemma BatchOperations_decrypt_all_finished_oracle_eq:
+forall u l1 l2 o1 o2 o3 o4 s1 s2 s1' s2' r1 r2 k1 k2,
+exec CryptoDiskLang u o1 s1
+(BatchOperations.decrypt_all k1 l1)  (Finished s1' r1) ->
+exec CryptoDiskLang u o2 s2
+(BatchOperations.decrypt_all k2 l2) (Finished s2' r2) ->
+o1 ++ o3 = o2 ++ o4 ->
+length l1 = length l2 ->
+o1 = o2.
+Proof.
+  induction l1; destruct l2; simpl; intros; try lia.
+  repeat invert_exec; eauto.
+  repeat invert_exec; cleanup; eauto.
+  repeat rewrite <- app_assoc in *; cleanup.
+  eapply IHl1 in H1; eauto.
+  subst; eauto.
+Qed.
+
+
+
+
+Lemma log_read_header_finished_oracle_eq:
+forall u o1 o2 o3 o4 s1 s2 s1' s2' r1 r2,
+exec CryptoDiskLang u o1 s1
+read_header  (Finished s1' r1) ->
+exec CryptoDiskLang u o2 s2
+read_header (Finished s2' r2) ->
+o1 ++ o3 = o2 ++ o4 ->
+o1 = o2.
+Proof.
+  Transparent read_header.
+  unfold read_header; intros.
+  cleanup; repeat invert_exec; simpl in *; cleanup;
+  eauto.
+  Opaque read_header.
+Qed.
+
+Lemma log_write_header_finished_oracle_eq:
+forall u o1 o2 o3 o4 s1 s2 s1' s2' r1 r2 h1 h2,
+exec CryptoDiskLang u o1 s1
+(write_header h1) (Finished s1' r1) ->
+exec CryptoDiskLang u o2 s2
+(write_header h2) (Finished s2' r2) ->
+o1 ++ o3 = o2 ++ o4 ->
+o1 = o2.
+Proof.
+  Transparent write_header.
+  unfold write_header; intros.
+  cleanup; repeat invert_exec; simpl in *; cleanup;
+  eauto.
+  Opaque write_header.
+Qed.
+
+Lemma log_update_header_finished_oracle_eq:
+forall u o1 o2 o3 o4 s1 s2 s1' s2' r1 r2 h1 h2,
+exec CryptoDiskLang u o1 s1
+(update_header h1) (Finished s1' r1) ->
+exec CryptoDiskLang u o2 s2
+(update_header h2) (Finished s2' r2) ->
+o1 ++ o3 = o2 ++ o4 ->
+o1 = o2.
+Proof.
+  Transparent update_header.
+  unfold update_header; intros.
+  cleanup; repeat invert_exec; simpl in *; cleanup;
+  eauto.
+  repeat rewrite <- app_assoc in *; cleanup.
+  eapply log_read_header_finished_oracle_eq in H; eauto.
+  cleanup.
+  eapply log_write_header_finished_oracle_eq in H3; eauto.
+  subst; eauto.
+  Opaque update_header.
+Qed.
+
+
+
+Lemma log_commit_txn_finished_oracle_eq:
+forall u o1 o2 o3 o4 s1 s2 s1' s2' r1 r2 a1 a2 v1 v2,
+exec CryptoDiskLang u o1 s1
+(commit_txn a1 v1)  (Finished s1' r1) ->
+exec CryptoDiskLang u o2 s2
+(commit_txn a2 v2) (Finished s2' r2) ->
+o1 ++ o3 = o2 ++ o4 ->
+length (a2 ++ v2) = length (a1 ++ v1) ->
+o1 = o2.
+Proof.
+  unfold commit_txn; intros.
+  cleanup; repeat invert_exec; simpl in *; cleanup;
+  eauto; try lia.
+  repeat rewrite <- app_assoc in *; cleanup.
+
+  eapply log_read_header_finished_oracle_eq in H; eauto; cleanup.
+  simpl in *; cleanup.
+
+  repeat rewrite <- app_assoc in *; cleanup.
+  eapply_fresh BatchOperations_encrypt_all_finished_oracle_eq in H13; eauto. 
+  cleanup.
+
+  eapply BatchOperations.encrypt_all_finished in H13.
+  eapply BatchOperations.encrypt_all_finished in H4.
+  cleanup.
+  repeat rewrite <- app_assoc in *; cleanup.
+  eapply_fresh BatchOperations_hash_all_finished_oracle_eq in H15; eauto. 
+  cleanup.
+
+  eapply BatchOperations.hash_all_finished in H15.
+  eapply BatchOperations.hash_all_finished in H6.
+  cleanup.
+  repeat rewrite <- app_assoc in *; cleanup.
+  eapply BatchOperations_write_consecutive_finished_oracle_eq in H16; eauto. 
+  cleanup.
+
+  repeat rewrite <- app_assoc in *; cleanup.
+  eapply log_update_header_finished_oracle_eq in H17; eauto.
+  subst; eauto.
+  all: repeat rewrite map_length; eauto. 
+Qed.
+
+Lemma log_commit_finished_oracle_eq:
+forall u o1 o2 o3 o4 s1 s2 s1' s2' r1 r2 a1 a2 v1 v2,
+exec CryptoDiskLang u o1 s1
+(commit a1 v1)  (Finished s1' r1) ->
+exec CryptoDiskLang u o2 s2
+(commit a2 v2) (Finished s2' r2) ->
+o1 ++ o3 = o2 ++ o4 ->
+length (a1 ++ v1) = length (a2 ++ v2) ->
+(log_length >=
+count
+  (current_part
+     (decode_header
+        (fst (snd s1 hdr_block_num)))) +
+(length a1 + length v1) <-> log_length >=
+count
+  (current_part
+     (decode_header
+        (fst (snd s2 hdr_block_num)))) +
+(length a2 + length v2)) ->
+o1 = o2.
+Proof.
+  Transparent commit.
+  unfold commit; intros.
+  cleanup; repeat invert_exec; simpl in *; cleanup;
+  eauto; try lia;
+  repeat rewrite <- app_assoc in *;
+  try eapply_fresh log_read_header_finished_oracle_eq in H; eauto;
+  subst; eauto; cleanup.
+  {
+    apply Nat.ltb_ge in D0.
+    apply Nat.ltb_lt in D.
+    Transparent read_header.
+    unfold read_header in *; repeat invert_exec; cleanup.
+    repeat cleanup_pairs; lia.
+    Opaque read_header.
+  }
+  {
+    apply Nat.ltb_ge in D.
+    apply Nat.ltb_lt in D0.
+    Transparent read_header.
+    unfold read_header in *; repeat invert_exec; cleanup.
+    repeat cleanup_pairs; lia.
+    Opaque read_header.
+  }
+  {
+    eapply log_commit_txn_finished_oracle_eq in H5; eauto.
+    cleanup; eauto.
+  }
+  Opaque commit.
+Qed.
+
+Lemma log_check_hash_finished_oracle_eq:
+forall u l1 l2 h1 h2 o1 o2 o3 o4 s1 s2 s1' s2' r1 r2,
+exec CryptoDiskLang u o1 s1
+(check_hash l1 h1) (Finished s1' r1) ->
+exec CryptoDiskLang u o2 s2
+(check_hash l2 h2) (Finished s2' r2) ->
+o1 ++ o3 = o2 ++ o4 ->
+length l1 = length l2 ->
+o1 = o2.
+Proof.
+  Transparent check_hash.
+  unfold check_hash; intros.
+  cleanup; repeat invert_exec; simpl in *; cleanup;
+  eauto; try lia;
+  repeat rewrite <- app_assoc in *;
+  try eapply_fresh BatchOperations_hash_all_finished_oracle_eq in H; eauto;
+  subst; eauto; cleanup.
+Qed.
+
+
+Lemma log_read_encrypted_log_finished_oracle_eq:
+forall u o1 o2 o3 o4 s1 s2 s1' s2' r1 r2,
+exec CryptoDiskLang u o1 s1
+read_encrypted_log (Finished s1' r1) ->
+exec CryptoDiskLang u o2 s2
+read_encrypted_log (Finished s2' r2) ->
+o1 ++ o3 = o2 ++ o4 ->
+o1 = o2.
+Proof.
+  Transparent read_encrypted_log.
+  unfold read_encrypted_log; intros.
+  cleanup; repeat invert_exec; simpl in *; cleanup;
+  eauto; try lia;
+  repeat rewrite <- app_assoc in *;
+  try eapply_fresh log_read_header_finished_oracle_eq in H; eauto;
+  subst; eauto; cleanup.
+  {
+      eapply_fresh BatchOperations_read_consecutive_finished_oracle_eq in H4; eauto. 
+      cleanup.
+      eapply_fresh log_check_hash_finished_oracle_eq in H5; eauto. 
+      cleanup; eauto.
+      all: admit.
+  }
+  {
+      eapply_fresh BatchOperations_read_consecutive_finished_oracle_eq in H4; eauto. 
+      cleanup.
+      eapply_fresh log_check_hash_finished_oracle_eq in H5; eauto. 
+      cleanup; eauto.
+
+      unfold check_hash in *; repeat invert_exec; try congruence.
+      (* Impossible case between related states. *)
+      all: admit.
+  }
+  {
+    admit. (* Impossible case between related states. *)
+  }
+  {
+    eapply_fresh BatchOperations_read_consecutive_finished_oracle_eq in H5.
+    2: apply H2. 
+    all: eauto. 
+    cleanup.
+
+    eapply_fresh log_check_hash_finished_oracle_eq in H6; eauto. 
+    cleanup; eauto.
+    eapply_fresh BatchOperations_read_consecutive_finished_oracle_eq in H7; eauto.
+    cleanup; eauto.
+    all: admit.
+  }
+  Opaque read_encrypted_log.
+Admitted.
+
+Lemma log_decrypt_txn_finished_oracle_eq:
+forall u txn_rec1 txn_rec2 l1 l2 o1 o2 o3 o4 s1 s2 s1' s2' r1 r2,
+exec CryptoDiskLang u o1 s1
+(decrypt_txn txn_rec1 l1) (Finished s1' r1) ->
+exec CryptoDiskLang u o2 s2
+(decrypt_txn txn_rec2 l2) (Finished s2' r2) ->
+o1 ++ o3 = o2 ++ o4 ->
+length
+  (firstn (addr_count txn_rec1 + data_count txn_rec1)
+     (skipn (start txn_rec1) l1)) =
+length
+  (firstn (addr_count txn_rec2 + data_count txn_rec2)
+     (skipn (start txn_rec2) l2)) ->
+o1 = o2.
+Proof.
+  unfold decrypt_txn; simpl; intros.
+  repeat invert_exec; eauto.
+  repeat rewrite <- app_assoc in *.
+  eapply BatchOperations_decrypt_all_finished_oracle_eq in H; eauto.
+  cleanup; eauto.
+Qed.
+
+
+Lemma log_apply_txn_finished_oracle_eq:
+forall u txn_rec1 txn_rec2 l1 l2 o1 o2 o3 o4 s1 s2 s1' s2' r1 r2,
+exec CryptoDiskLang u o1 s1
+(apply_txn txn_rec1 l1) (Finished s1' r1) ->
+exec CryptoDiskLang u o2 s2
+(apply_txn txn_rec2 l2) (Finished s2' r2) ->
+o1 ++ o3 = o2 ++ o4 ->
+o1 = o2.
+Proof.
+  Transparent apply_txn.
+  unfold apply_txn; simpl; intros.
+  repeat invert_exec; eauto.
+  repeat rewrite <- app_assoc in *.
+  eapply_fresh log_decrypt_txn_finished_oracle_eq in H; eauto.
+  cleanup.
+  eapply BatchOperations_write_batch_finished_oracle_eq in H3; eauto.
+  cleanup; eauto.
+Admitted.
+
+
+Lemma log_apply_txns_finished_oracle_eq:
+forall u txn_recs1 txn_recs2 l1 l2 o1 o2 o3 o4 s1 s2 s1' s2' r1 r2,
+exec CryptoDiskLang u o1 s1
+(apply_txns txn_recs1 l1) (Finished s1' r1) ->
+exec CryptoDiskLang u o2 s2
+(apply_txns txn_recs2 l2) (Finished s2' r2) ->
+o1 ++ o3 = o2 ++ o4 ->
+length txn_recs1 = length txn_recs2 ->
+o1 = o2.
+Proof.
+  Transparent apply_txns.
+  induction txn_recs1; destruct txn_recs2; simpl; intros; try lia.
+  repeat invert_exec; eauto.
+  repeat invert_exec; eauto.
+  repeat rewrite <- app_assoc in *.
+  eapply log_apply_txn_finished_oracle_eq in H; eauto.
+  cleanup.
+  eapply IHtxn_recs1 in H3; eauto.
+  cleanup; eauto.
+Qed.
+
+Lemma log_decrypt_txns_finished_oracle_eq:
+forall u txn_recs1 txn_recs2 l1 l2 o1 o2 o3 o4 s1 s2 s1' s2' r1 r2,
+exec CryptoDiskLang u o1 s1
+(decrypt_txns txn_recs1 l1) (Finished s1' r1) ->
+exec CryptoDiskLang u o2 s2
+(decrypt_txns txn_recs2 l2) (Finished s2' r2) ->
+o1 ++ o3 = o2 ++ o4 ->
+length txn_recs1 = length txn_recs2 ->
+o1 = o2.
+Proof.
+  Transparent apply_txns.
+  induction txn_recs1; destruct txn_recs2; simpl; intros; try lia.
+  repeat invert_exec; eauto.
+  repeat invert_exec; eauto.
+  repeat rewrite <- app_assoc in *.
+  eapply log_decrypt_txn_finished_oracle_eq in H; eauto.
+  cleanup.
+  eapply IHtxn_recs1 in H3; eauto.
+  cleanup; eauto.
+Admitted.
+
+
+Lemma log_flush_txns_finished_oracle_eq:
+forall u txn_recs1 txn_recs2 l1 l2 o1 o2 o3 o4 s1 s2 s1' s2' r1 r2,
+exec CryptoDiskLang u o1 s1
+(flush_txns txn_recs1 l1) (Finished s1' r1) ->
+exec CryptoDiskLang u o2 s2
+(flush_txns txn_recs2 l2) (Finished s2' r2) ->
+o1 ++ o3 = o2 ++ o4 ->
+length txn_recs1 = length txn_recs2 ->
+o1 = o2.
+Proof.
+  Transparent flush_txns.
+  unfold flush_txns; intros.
+  cleanup; repeat invert_exec; simpl in *; cleanup;
+  eauto; try lia;
+  repeat rewrite <- app_assoc in *.
+  eapply log_apply_txns_finished_oracle_eq in H; eauto.
+  simpl in *; cleanup.
+  repeat rewrite <- app_assoc in *.
+  eapply log_update_header_finished_oracle_eq in H9; eauto.
+  cleanup; eauto.
+Qed.
+
+Lemma log_apply_log_finished_oracle_eq:
+forall u o1 o2 o3 o4 s1 s2 s1' s2' r1 r2,
+exec CryptoDiskLang u o1 s1
+apply_log (Finished s1' r1) ->
+exec CryptoDiskLang u o2 s2
+apply_log (Finished s2' r2) ->
+o1 ++ o3 = o2 ++ o4 ->
+o1 = o2.
+Proof.
+  Transparent apply_log.
+  unfold apply_log; intros.
+  cleanup; repeat invert_exec; simpl in *; cleanup;
+  eauto; try lia;
+  repeat rewrite <- app_assoc in *;
+  try eapply_fresh log_read_header_finished_oracle_eq in H0; eauto;
+  subst; eauto; cleanup.
+  eapply log_read_encrypted_log_finished_oracle_eq in H; eauto.
+  cleanup.
+  eapply log_flush_txns_finished_oracle_eq in H3; eauto.
+  cleanup; eauto.
+Admitted.
+
+
+Lemma log_recover_finished_oracle_eq:
+forall u o1 o2 o3 o4 s1 s2 s1' s2' r1 r2,
+exec CryptoDiskLang u o1 s1
+Log.recover (Finished s1' r1) ->
+exec CryptoDiskLang u o2 s2
+Log.recover (Finished s2' r2) ->
+o1 ++ o3 = o2 ++ o4 ->
+o1 = o2.
+Proof.
+  Transparent Log.recover.
+  unfold Log.recover; intros.
+  cleanup; repeat invert_exec; simpl in *; cleanup;
+  eauto; try lia;
+  repeat rewrite <- app_assoc in *;
+  try eapply_fresh log_read_header_finished_oracle_eq in H0; eauto;
+  subst; eauto; cleanup.
+  eapply log_read_encrypted_log_finished_oracle_eq in H; eauto.
+  cleanup.
+  eapply log_write_header_finished_oracle_eq in H6; eauto.
+  cleanup.
+  simpl in *; cleanup.
+  eapply log_decrypt_txns_finished_oracle_eq in H8; eauto.
+  cleanup; eauto.
+Admitted.
+
+Lemma log_init_finished_oracle_eq:
+forall u l1 l2 o1 o2 o3 o4 s1 s2 s1' s2' r1 r2 ,
+exec CryptoDiskLang u o1 s1
+(Log.init l1)  (Finished s1' r1) ->
+exec CryptoDiskLang u o2 s2
+(Log.init l2) (Finished s2' r2) ->
+o1 ++ o3 = o2 ++ o4 ->
+length l1 = length l2 ->
+o1 = o2.
+Proof.
+  Transparent Log.init.
+  unfold Log.init; intros.
+  cleanup; repeat invert_exec; simpl in *; cleanup;
+  eauto.
+  repeat rewrite <- app_assoc in *.
+  eapply log_write_header_finished_oracle_eq in H; eauto.
+  cleanup.
+  eapply BatchOperations_write_batch_finished_oracle_eq in H6; eauto.
+  cleanup; eauto.
+  all: repeat rewrite map_length; eauto.
+Qed.
+
+
+Lemma read_finished_oracle_eq:
+forall u o1 o2 o3 o4 s1 s2 s1' s2' r1 r2 a1 a2,
+exec CachedDiskLang u o1 s1
+(read a1)  (Finished s1' r1) ->
+exec CachedDiskLang u o2 s2
+(read a2) (Finished s2' r2) ->
+o1 ++ o3 = o2 ++ o4 ->
+o1 = o2.
+Proof.
+  unfold read; intros.
+  cleanup; repeat invert_exec; simpl in *; cleanup;
+  eauto.
+Qed.
+
+
+
+Lemma write_batch_to_cache_finished_oracle_eq:
+forall u l1 l2 l3 l4 o1 o2 o3 o4 s1 s2 s1' s2' r1 r2,
+exec CachedDiskLang u o1 s1
+(LogCache.write_batch_to_cache l1 l3)  (Finished s1' r1) ->
+exec CachedDiskLang u o2 s2
+(LogCache.write_batch_to_cache l2 l4) (Finished s2' r2) ->
+o1 ++ o3 = o2 ++ o4 ->
+length l1 = length l2 ->
+o1 = o2.
+Proof.
+  induction l1; destruct l2; simpl in *; intros; try lia;
+  cleanup; repeat invert_exec; simpl in *; cleanup;
+  eauto.
+  repeat rewrite <- app_assoc in *.
+  eapply IHl1 in H3; eauto.
+  cleanup; eauto.
+Qed.
+
+Lemma write_lists_to_cache_finished_oracle_eq:
+forall u l1 l2 o1 o2 o3 o4 s1 s2 s1' s2' r1 r2,
+exec CachedDiskLang u o1 s1
+(LogCache.write_lists_to_cache l1)  (Finished s1' r1) ->
+exec CachedDiskLang u o2 s2
+(LogCache.write_lists_to_cache l2) (Finished s2' r2) ->
+o1 ++ o3 = o2 ++ o4 ->
+length l1 = length l2 ->
+o1 = o2.
+Proof.
+  induction l1; destruct l2; simpl in *; intros; try lia;
+  cleanup; repeat invert_exec; simpl in *; cleanup;
+  eauto.
+  repeat rewrite <- app_assoc in *.
+  eapply write_batch_to_cache_finished_oracle_eq in H; eauto.
+  cleanup.
+  eapply IHl1 in H3; eauto.
+  subst; eauto.
+Admitted.
+
+
+Lemma recover_finished_oracle_eq:
+forall u o1 o2 o3 o4 s1 s2 s1' s2' r1 r2,
+exec CachedDiskLang u o1 s1
+recover  (Finished s1' r1) ->
+exec CachedDiskLang u o2 s2
+recover (Finished s2' r2) ->
+o1 ++ o3 = o2 ++ o4 ->
+o1 = o2.
+Proof.
+  unfold recover; intros.
+  cleanup; repeat invert_exec; simpl in *; cleanup;
+  eauto.
+  repeat rewrite <- app_assoc in *.
+  eapply log_recover_finished_oracle_eq in H10; eauto.
+  cleanup.
+  eapply write_lists_to_cache_finished_oracle_eq in H8; eauto.
+  cleanup; eauto.
+Admitted.
+
+
+Lemma init_finished_oracle_eq:
+forall u l1 l2 o1 o2 o3 o4 s1 s2 s1' s2' r1 r2 ,
+exec CachedDiskLang u o1 s1
+(init l1)  (Finished s1' r1) ->
+exec CachedDiskLang u o2 s2
+(init l2) (Finished s2' r2) ->
+o1 ++ o3 = o2 ++ o4 ->
+length l1 = length l2 ->
+o1 = o2.
+Proof.
+  unfold init; intros.
+  cleanup; repeat invert_exec; simpl in *; cleanup;
+  eauto.
+  apply map_ext_eq_prefix in H10; eauto; cleanup.
+  eapply log_init_finished_oracle_eq in H8; eauto.
+  subst; eauto.
+  repeat rewrite combine_length_eq.
+  all: repeat rewrite map_length; eauto.
+  repeat constructor.
+  exact key0.
+  intros; cleanup; intuition congruence.
+Qed.
+
+Lemma write_finished_oracle_eq:
+forall u o1 o2 o3 o4 s1 s2 s1' s2' r1 r2 a1 a2 v1 v2,
+exec CachedDiskLang u o1 s1
+(write a1 v1)  (Finished s1' r1) ->
+exec CachedDiskLang u o2 s2
+(write a2 v2) (Finished s2' r2) ->
+o1 ++ o3 = o2 ++ o4 ->
+o1 = o2.
+Proof.
+  unfold write; intros.
+  cleanup; repeat invert_exec; simpl in *; cleanup;
+  eauto.
+Admitted.
+
+
+
+(* Finished Not Crashed proofs*)
+Lemma BatchOperations_read_consecutive_finished_not_crashed:
+forall u n1 n2 st1 st2 o1 o2 o3 o4 s1 s2 s1' s2' r1,
+exec CryptoDiskLang u o1 s1
+(BatchOperations.read_consecutive st1 n1) (Finished s1' r1) ->
+o1 ++ o3 = o2 ++ o4 ->
+n1 = n2 ->
+~exec CryptoDiskLang u o2 s2
+(BatchOperations.read_consecutive st2 n2) (Crashed s2').
+Proof.
+  unfold not; induction n1; destruct n2; simpl; intros; cleanup;
+  cleanup; repeat invert_exec; simpl in *; cleanup;
+  eauto;
+  repeat (try split_ors; cleanup;
+  repeat invert_exec; simpl in *; cleanup;
+  eauto).
+  repeat rewrite <- app_assoc in *.
+  eapply IHn1.
+  eauto.
+  3: eauto.
+  all: eauto.
+  repeat rewrite <- app_assoc in *.
+  eapply BatchOperations_read_consecutive_finished_oracle_eq in H; eauto. 
+  cleanup; simpl in *; cleanup.
+  lia.
+Qed.
+
+Lemma BatchOperations_hash_all_finished_not_crashed:
+forall u n1 n2 st1 st2 o1 o2 o3 o4 s1 s2 s1' s2' r1,
+exec CryptoDiskLang u o1 s1
+(BatchOperations.hash_all st1 n1) (Finished s1' r1) ->
+o1 ++ o3 = o2 ++ o4 ->
+length n1 = length n2 ->
+~exec CryptoDiskLang u o2 s2
+(BatchOperations.hash_all st2 n2) (Crashed s2').
+Proof.
+  unfold not; induction n1; destruct n2; simpl; intros; cleanup;
+  cleanup; repeat invert_exec; simpl in *; cleanup;
+  eauto;
+  repeat (try split_ors; cleanup;
+  repeat invert_exec; simpl in *; cleanup;
+  eauto).
+  repeat rewrite <- app_assoc in *.
+  eapply IHn1.
+  eauto.
+  3: eauto.
+  all: eauto.
+  repeat rewrite <- app_assoc in *.
+  eapply BatchOperations_hash_all_finished_oracle_eq in H; eauto. 
+  cleanup; simpl in *; cleanup.
+  lia.
+Qed.
+
+Lemma BatchOperations_decrypt_all_finished_not_crashed:
+forall u n1 n2 st1 st2 o1 o2 o3 o4 s1 s2 s1' s2' r1,
+exec CryptoDiskLang u o1 s1
+(BatchOperations.decrypt_all st1 n1) (Finished s1' r1) ->
+o1 ++ o3 = o2 ++ o4 ->
+length n1 = length n2 ->
+~exec CryptoDiskLang u o2 s2
+(BatchOperations.decrypt_all st2 n2) (Crashed s2').
+Proof.
+  unfold not; induction n1; destruct n2; simpl; intros; cleanup;
+  cleanup; repeat invert_exec; simpl in *; cleanup;
+  eauto;
+  repeat (try split_ors; cleanup;
+  repeat invert_exec; simpl in *; cleanup;
+  eauto).
+  repeat rewrite <- app_assoc in *.
+  eapply IHn1.
+  eauto.
+  3: eauto.
+  all: eauto.
+  repeat rewrite <- app_assoc in *.
+  eapply BatchOperations_decrypt_all_finished_oracle_eq in H; eauto. 
+  cleanup; simpl in *; cleanup.
+  lia.
+Qed.
+
+Lemma BatchOperations_write_batch_finished_not_crashed:
+forall u st1 st2 n1 n2 o1 o2 o3 o4 s1 s2 s1' s2' r1,
+exec CryptoDiskLang u o1 s1
+(BatchOperations.write_batch st1 n1) (Finished s1' r1) ->
+o1 ++ o3 = o2 ++ o4 ->
+length st1 = length st2 ->
+length n1 = length n2 ->
+~exec CryptoDiskLang u o2 s2
+(BatchOperations.write_batch st2 n2) (Crashed s2').
+Proof.
+  unfold not; induction st1; destruct st2; simpl; intros; cleanup;
+  cleanup; repeat invert_exec; simpl in *; cleanup;
+  eauto;
+  repeat (try split_ors; cleanup;
+  repeat invert_exec; simpl in *; cleanup;
+  eauto).
+  repeat rewrite <- app_assoc in *.
+  simpl in *.
+  eapply IHst1.
+  eauto.
+  4: eauto.
+  all: eauto.
+
+  repeat rewrite <- app_assoc in *.
+  eapply BatchOperations_write_batch_finished_oracle_eq in H; eauto. 
+  cleanup; simpl in *; cleanup.
+  all: lia.
+Qed.
+
+
+Lemma log_read_header_finished_not_crashed:
+forall u o1 o2 o3 o4 s1 s2 s1' s2' r1,
+exec CryptoDiskLang u o1 s1
+read_header (Finished s1' r1) ->
+o1 ++ o3 = o2 ++ o4 ->
+~exec CryptoDiskLang u o2 s2
+read_header (Crashed s2').
+Proof.
+  Transparent read_header.
+  unfold read_header, not; intros.
+  cleanup; repeat invert_exec; simpl in *; cleanup;
+  eauto;
+  repeat (try split_ors; cleanup;
+  repeat invert_exec; simpl in *; cleanup;
+  eauto).
+  Opaque read_header.
+Qed.
+
+Lemma log_check_hash_finished_not_crashed:
+forall u l1 l2 h1 h2 o1 o2 o3 o4 s1 s2 s1' s2' r1,
+exec CryptoDiskLang u o1 s1
+(check_hash l1 h1) (Finished s1' r1) ->
+o1 ++ o3 = o2 ++ o4 ->
+length l1 = length l2 ->
+~exec CryptoDiskLang u o2 s2
+(check_hash l2 h2) (Crashed s2').
+Proof.
+  unfold check_hash, not; intros.
+  cleanup; repeat invert_exec; simpl in *; cleanup;
+  eauto.
+
+  repeat rewrite <- app_assoc in *.
+    try split_ors; cleanup;
+    repeat invert_exec; simpl in *; cleanup;
+    eauto.
+    eapply BatchOperations_hash_all_finished_not_crashed; eauto.
+    
+    repeat rewrite <- app_assoc in *.
+    eapply BatchOperations_hash_all_finished_oracle_eq in H; eauto; cleanup.
+    try split_ors; cleanup;
+    repeat invert_exec; simpl in *; cleanup;
+    eauto.
+
+
+    repeat rewrite <- app_assoc in *.
+    eapply BatchOperations_hash_all_finished_oracle_eq in H; eauto; cleanup.
+    try split_ors; cleanup;
+    repeat invert_exec; simpl in *; cleanup;
+    eauto.
+
+    repeat rewrite <- app_assoc in *.
+    try split_ors; cleanup;
+    repeat invert_exec; simpl in *; cleanup;
+    eauto.
+    eapply BatchOperations_hash_all_finished_not_crashed; eauto.
+
+    repeat rewrite <- app_assoc in *.
+    eapply BatchOperations_hash_all_finished_oracle_eq in H; eauto; cleanup.
+    try split_ors; cleanup;
+    repeat invert_exec; simpl in *; cleanup;
+    eauto.
+
+
+    repeat rewrite <- app_assoc in *.
+    eapply BatchOperations_hash_all_finished_oracle_eq in H; eauto; cleanup.
+    try split_ors; cleanup;
+    repeat invert_exec; simpl in *; cleanup;
+    eauto.
+Qed.
+
+Lemma log_read_encrypted_log_finished_not_crashed:
+forall u o1 o2 o3 o4 s1 s2 s1' s2' r1,
+exec CryptoDiskLang u o1 s1
+read_encrypted_log (Finished s1' r1) ->
+o1 ++ o3 = o2 ++ o4 ->
+~exec CryptoDiskLang u o2 s2
+read_encrypted_log (Crashed s2').
+Proof.
+  Transparent read_encrypted_log.
+  unfold read_encrypted_log, not; intros.
+  cleanup; repeat invert_exec; simpl in *; cleanup;
+  eauto.
+  {
+    repeat rewrite <- app_assoc in *.
+    try split_ors; cleanup;
+    repeat invert_exec; simpl in *; cleanup;
+    eauto.
+    eapply log_read_header_finished_not_crashed; eauto.
+
+    repeat rewrite <- app_assoc in *.
+    eapply log_read_header_finished_oracle_eq in H; eauto; cleanup.
+    try split_ors; cleanup;
+    repeat invert_exec; simpl in *; cleanup;
+    eauto.
+    eapply BatchOperations_read_consecutive_finished_not_crashed.
+    eauto.
+    3:eauto.
+    all: eauto.
+    shelve.
+
+    repeat rewrite <- app_assoc in *.
+    eapply BatchOperations_read_consecutive_finished_oracle_eq in H2; eauto; cleanup.
+    try split_ors; cleanup;
+    repeat invert_exec; simpl in *; cleanup;
+    eauto.
+       eapply log_check_hash_finished_not_crashed.
+    eauto.
+    3:eauto.
+    all: eauto.
+    shelve.
+
+    repeat rewrite <- app_assoc in *.
+    eapply log_check_hash_finished_oracle_eq in H3; eauto; cleanup.
+    try split_ors; cleanup;
+    repeat invert_exec; simpl in *; cleanup;
+    eauto.
+    shelve.
+
+    shelve.
+    shelve.
+  }
+  {
+    repeat rewrite <- app_assoc in *.
+    try split_ors; cleanup;
+    repeat invert_exec; simpl in *; cleanup;
+    eauto.
+    eapply log_read_header_finished_not_crashed; eauto.
+
+    repeat rewrite <- app_assoc in *.
+    eapply log_read_header_finished_oracle_eq in H; eauto; cleanup.
+    try split_ors; cleanup;
+    repeat invert_exec; simpl in *; cleanup;
+    eauto.
+    eapply BatchOperations_read_consecutive_finished_not_crashed.
+    apply H2.
+    3:eauto.
+    all: eauto.
+    shelve.
+
+    repeat rewrite <- app_assoc in *.
+    eapply BatchOperations_read_consecutive_finished_oracle_eq in H2; eauto; cleanup.
+    try split_ors; cleanup;
+    repeat invert_exec; simpl in *; cleanup;
+    eauto.
+    eapply log_check_hash_finished_not_crashed.
+    eauto.
+    3:eauto.
+    all: eauto.
+    shelve.
+
+    shelve.
+
+    repeat rewrite <- app_assoc in *.
+    eapply log_check_hash_finished_oracle_eq in H3; eauto; cleanup.
+    try split_ors; cleanup;
+    repeat invert_exec; simpl in *; cleanup;
+    eauto.
+
+    try split_ors; cleanup;
+    repeat invert_exec; simpl in *; cleanup;
+    eauto.
+    eapply BatchOperations_read_consecutive_finished_not_crashed.
+    4: eauto.
+    2: eauto.
+    all: eauto.
+    shelve.
+
+    repeat rewrite <- app_assoc in *.
+    eapply BatchOperations_read_consecutive_finished_oracle_eq in H4; eauto; cleanup.
+    simpl in *; cleanup.
+    shelve.
+    shelve.
+    shelve.
+  }
+  Unshelve.
+Admitted.
+
+Lemma log_write_header_finished_not_crashed:
+forall u o1 o2 o3 o4 s1 s2 s1' s2' r1 h1 h2,
+exec CryptoDiskLang u o1 s1
+(write_header h1) (Finished s1' r1) ->
+o1 ++ o3 = o2 ++ o4 ->
+~exec CryptoDiskLang u o2 s2
+(write_header h2) (Crashed s2').
+Proof.
+  Transparent write_header.
+  unfold write_header, not; intros.
+  cleanup; repeat invert_exec; simpl in *; cleanup;
+  eauto;
+  repeat (try split_ors; cleanup;
+  repeat invert_exec; simpl in *; cleanup;
+  eauto).
+Qed.
+
+Lemma log_decrypt_txn_finished_not_crashed:
+forall u rec1 rec2 l1 l2 o1 o2 o3 o4 s1 s2 s1' s2' r1,
+exec CryptoDiskLang u o1 s1
+(decrypt_txn rec1 l1) (Finished s1' r1) ->
+o1 ++ o3 = o2 ++ o4 ->
+length (firstn (addr_count rec1 + data_count rec1) (skipn (start rec1) l1)) =
+length (firstn (addr_count rec2 + data_count rec2) (skipn (start rec2) l2)) ->
+~exec CryptoDiskLang u o2 s2
+(decrypt_txn rec2 l2) (Crashed s2').
+Proof.
+  unfold decrypt_txn, not;  intros. 
+  cleanup; repeat invert_exec; simpl in *; cleanup;
+  eauto;
+  repeat (try split_ors; cleanup;
+  repeat invert_exec; simpl in *; cleanup;
+  eauto).
+  repeat rewrite <- app_assoc in *.
+  eapply BatchOperations_decrypt_all_finished_not_crashed. 
+  4: eauto.
+  eauto.
+  all: eauto.
+
+  repeat rewrite <- app_assoc in *.
+  eapply BatchOperations_decrypt_all_finished_oracle_eq in H; eauto. 
+  cleanup; simpl in *; cleanup.
+Qed.
+
+Lemma log_decrypt_txns_finished_not_crashed:
+forall u recs1 recs2 l1 l2 o1 o2 o3 o4 s1 s2 s1' s2' r1,
+exec CryptoDiskLang u o1 s1
+(decrypt_txns recs1 l1) (Finished s1' r1) ->
+o1 ++ o3 = o2 ++ o4 ->
+length recs1 = length recs2 ->
+~exec CryptoDiskLang u o2 s2
+(decrypt_txns recs2 l2) (Crashed s2').
+Proof.
+  unfold not; 
+  induction recs1; destruct recs2; simpl; intros; try lia.
+  cleanup; repeat invert_exec; simpl in *; cleanup;
+  eauto;
+  repeat (try split_ors; cleanup;
+  repeat invert_exec; simpl in *; cleanup;
+  eauto).
+
+  cleanup; repeat invert_exec; simpl in *; cleanup;
+  eauto;
+  repeat (try split_ors; cleanup;
+  repeat invert_exec; simpl in *; cleanup;
+  eauto).
+
+  repeat rewrite <- app_assoc in *.
+  eapply log_decrypt_txn_finished_not_crashed. 
+  4: eauto.
+  eauto.
+  all: eauto.
+  shelve.
+
+  repeat rewrite <- app_assoc in *.
+  eapply log_decrypt_txn_finished_oracle_eq in H; eauto. 
+  cleanup; simpl in *; cleanup.
+  eapply IHrecs1.
+  4: eauto.
+  eauto.
+  all: eauto.
+  shelve.
+
+  repeat rewrite <- app_assoc in *.
+  eapply log_decrypt_txn_finished_oracle_eq in H; eauto. 
+  cleanup; simpl in *; cleanup.
+  repeat rewrite <- app_assoc in *.
+  eapply log_decrypt_txns_finished_oracle_eq in H3; eauto. 
+  cleanup; simpl in *; cleanup.
+  lia.
+  shelve.
+Admitted.
+
+
+Lemma log_recover_finished_not_crashed:
+forall u o1 o2 o3 o4 s1 s2 s1' s2' r1,
+exec CryptoDiskLang u o1 s1
+Log.recover (Finished s1' r1) ->
+o1 ++ o3 = o2 ++ o4 ->
+~exec CryptoDiskLang u o2 s2
+Log.recover (Crashed s2').
+Proof.
+  unfold Log.recover, not; intros.
+  cleanup; repeat invert_exec; simpl in *; cleanup;
+  eauto;
+  repeat (try split_ors; cleanup;
+  repeat invert_exec; simpl in *; cleanup;
+  eauto).
+
+  repeat rewrite <- app_assoc in *.
+  eapply log_read_encrypted_log_finished_not_crashed in H; eauto.
+  
+
+  repeat rewrite <- app_assoc in *.
+  eapply log_read_encrypted_log_finished_oracle_eq in H; eauto. 
+  cleanup; simpl in *; cleanup.
+  eapply log_write_header_finished_not_crashed; eauto.
+  
+  repeat rewrite <- app_assoc in *.
+  eapply log_read_encrypted_log_finished_oracle_eq in H; eauto. 
+  cleanup; simpl in *; cleanup.
+  repeat rewrite <- app_assoc in *.
+  eapply log_write_header_finished_oracle_eq in H2; eauto. 
+  cleanup; simpl in *; cleanup.
+
+
+  repeat rewrite <- app_assoc in *.
+  eapply log_read_encrypted_log_finished_oracle_eq in H; eauto. 
+  cleanup; simpl in *; cleanup.
+  repeat rewrite <- app_assoc in *.
+  eapply log_write_header_finished_oracle_eq in H2; eauto. 
+  cleanup; simpl in *; cleanup.
+  eapply log_decrypt_txns_finished_not_crashed. 
+  4: eauto.
+  eauto.
+  all: eauto.
+  shelve.
+Admitted.
+
+
+Lemma log_init_finished_not_crashed:
+forall u l1 l2 o1 o2 o3 o4 s1 s2 s1' s2' r1,
+exec CryptoDiskLang u o1 s1
+(Log.init l1) (Finished s1' r1) ->
+o1 ++ o3 = o2 ++ o4 ->
+length l1 = length l2 ->
+~exec CryptoDiskLang u o2 s2
+(Log.init l2) (Crashed s2').
+Proof.
+  unfold Log.init, not; intros.
+  cleanup; repeat invert_exec; simpl in *; cleanup;
+  eauto;
+  repeat (try split_ors; cleanup;
+  repeat invert_exec; simpl in *; cleanup;
+  eauto).
+
+  repeat rewrite <- app_assoc in *.
+  eapply log_write_header_finished_not_crashed in H; eauto.
+  
+
+  repeat rewrite <- app_assoc in *.
+  eapply log_write_header_finished_oracle_eq in H; eauto. 
+  cleanup; simpl in *; cleanup.
+  eapply BatchOperations_write_batch_finished_not_crashed. 
+  eauto.
+  4: eauto.
+  all: repeat rewrite map_length; eauto.
+  
+
+  repeat rewrite <- app_assoc in *.
+  eapply log_write_header_finished_oracle_eq in H; eauto. 
+  cleanup; simpl in *; cleanup.
+  repeat rewrite <- app_assoc in *.
+  eapply BatchOperations_write_batch_finished_oracle_eq in H3; eauto. 
+  cleanup; simpl in *; cleanup.
+  all: repeat rewrite map_length; eauto.
+Qed.
+
+
+
+
+Lemma write_batch_to_cache_finished_not_crashed:
+forall u a1 a2 v1 v2 o1 o2 o3 o4 s1 s2 s1' s2' r1,
+exec CachedDiskLang u o1 s1
+(LogCache.write_batch_to_cache a1 v1)  (Finished s1' r1) ->
+o1 ++ o3 = o2 ++ o4 ->
+~exec CachedDiskLang u o2 s2
+(LogCache.write_batch_to_cache a2 v2) (Crashed s2').
+Proof.
+  unfold not; induction a1; destruct a2; 
+  simpl; intros; try lia;
+  cleanup; repeat invert_exec; simpl in *; cleanup;
+  eauto;
+  repeat (try split_ors; cleanup;
+  repeat invert_exec; simpl in *; cleanup;
+  eauto).
+Qed.
+
+
+Lemma write_lists_to_cache_finished_not_crashed:
+forall u a1 a2 o1 o2 o3 o4 s1 s2 s1' s2' r1,
+exec CachedDiskLang u o1 s1
+(LogCache.write_lists_to_cache a1)  (Finished s1' r1) ->
+o1 ++ o3 = o2 ++ o4 ->
+length a1 = length a2 ->
+~exec CachedDiskLang u o2 s2
+(LogCache.write_lists_to_cache a2) (Crashed s2').
+Proof.
+  unfold not; induction a1; destruct a2; 
+  simpl; intros; try lia;
+  cleanup; repeat invert_exec; simpl in *; cleanup;
+  eauto;
+  repeat (try split_ors; cleanup;
+  repeat invert_exec; simpl in *; cleanup;
+  eauto).
+
+  repeat rewrite <- app_assoc in *.
+  eapply write_batch_to_cache_finished_not_crashed; eauto.
+
+  repeat rewrite <- app_assoc in *.
+  eapply write_batch_to_cache_finished_oracle_eq in H; eauto.
+  cleanup; eauto.
+  shelve.
+Admitted.
+
+Lemma read_finished_not_crashed:
+forall u o1 o2 o3 o4 s1 s2 s1' s2' r1 a1 a2,
+exec CachedDiskLang u o1 s1
+(read a1)  (Finished s1' r1) ->
+o1 ++ o3 = o2 ++ o4 ->
+~exec CachedDiskLang u o2 s2
+(read a2) (Crashed s2').
+Proof.
+  unfold read, not; intros.
+  cleanup; repeat invert_exec; simpl in *; cleanup;
+  eauto;
+  repeat (try split_ors; cleanup;
+  repeat invert_exec; simpl in *; cleanup;
+  eauto).
+Qed.
+
+Opaque Log.recover.
+Lemma recover_finished_not_crashed:
+forall u o1 o2 o3 o4 s1 s2 s1' s2' r1,
+exec CachedDiskLang u o1 s1
+recover (Finished s1' r1) ->
+o1 ++ o3 = o2 ++ o4 ->
+~exec CachedDiskLang u o2 s2
+recover (Crashed s2').
+Proof.
+  unfold recover, not; intros.
+  cleanup; repeat invert_exec; simpl in *; cleanup;
+  eauto;
+  repeat (try split_ors; cleanup;
+  repeat invert_exec; simpl in *; cleanup;
+  eauto).
+
+  repeat rewrite <- app_assoc in *.
+  eapply map_ext_eq_prefix in H2.
+  cleanup.
+  eapply log_recover_finished_not_crashed; eauto.
+  solve [repeat constructor].
+  intros; cleanup; intuition congruence.
+
+  repeat rewrite <- app_assoc in *.
+  eapply_fresh map_ext_eq_prefix in H2.
+  cleanup.
+  eapply log_recover_finished_oracle_eq in H6; eauto.
+  cleanup.
+  eapply write_lists_to_cache_finished_not_crashed.
+  4: eauto.
+  eauto.
+  all: eauto.
+  shelve.
+  solve [repeat constructor].
+  intros; cleanup; intuition congruence.
+Admitted.
+
+Opaque Log.init.
+Lemma init_finished_not_crashed:
+forall u o1 o2 o3 o4 s1 s2 s1' s2' r1 a1 a2,
+exec CachedDiskLang u o1 s1
+(init a1)  (Finished s1' r1) ->
+o1 ++ o3 = o2 ++ o4 ->
+length a1 = length a2 ->
+~exec CachedDiskLang u o2 s2
+(init a2) (Crashed s2').
+Proof.
+  unfold init, not; intros.
+  cleanup; repeat invert_exec; simpl in *; cleanup;
+  eauto.
+  repeat (try split_ors; cleanup;
+  repeat invert_exec; simpl in *; cleanup;
+  eauto).
+
+  eapply map_ext_eq_prefix in H8; cleanup.
+  eapply log_init_finished_not_crashed. 
+  eauto.
+  3: eauto.
+  all: eauto.
+  repeat rewrite combine_length_eq; eauto.
+  all: repeat rewrite map_length; eauto.
+  solve [repeat econstructor].
+  intros; cleanup; intuition congruence.
+Qed.
+
+Opaque apply_log commit.
+Lemma write_finished_not_crashed:
+forall u o1 o2 o3 o4 s1 s2 s1' s2' r1 a1 a2 v1 v2,
+exec CachedDiskLang u o1 s1
+(write a1 v1)  (Finished s1' r1) ->
+o1 ++ o3 = o2 ++ o4 ->
+~exec CachedDiskLang u o2 s2
+(write a2 v2) (Crashed s2').
+Proof. Admitted.
+(*
+  unfold write, not; intros.
+  cleanup; repeat invert_exec; simpl in *; cleanup;
+  eauto;
+  repeat (try split_ors; cleanup;
+  repeat invert_exec; simpl in *; cleanup;
+  eauto).
+*)
