src/Noninterference/LoggedDisk/ATCD_ORS_Common.v
@@ -1,0 +1,1743 @@
+Require Import Eqdep Lia Framework FSParameters FileDiskLayer. (* LoggedDiskLayer TransactionCacheLayer TransactionalDiskLayer. *)
+Require Import FileDiskNoninterference LoggedDiskRefinement.
+Require Import (*HSS*) ATCDLayer ATCDSimulation ATCDAOE FinishedNotCrashed.
+Import FileDiskLayer.
+
+Ltac unify_execs_prefix :=
+  match goal with 
+  | [ H: Language.exec' ?u ?o1 ?s ?p (Finished _ _),
+      H0: Language.exec' ?u ?o2 ?s ?p (Finished _ _),
+      H1: ?o1 ++ _ = ?o2 ++ _ |- _] =>
+      eapply exec_finished_deterministic_prefix in H; [|apply H0| apply H1]
+  | [ H: Language.exec' ?u ?o1 ?s ?p (Finished _ _),
+      H0: exec _ ?u ?o2 ?s ?p (Finished _ _),
+      H1: ?o1 ++ _ = ?o2 ++ _ |- _] =>
+      eapply exec_finished_deterministic_prefix in H; [|apply H0| apply H1]
+  | [ H: exec _ ?u ?o1 ?s ?p (Finished _ _),
+      H0: exec _ ?u ?o2 ?s ?p (Finished _ _),
+      H1: ?o1 ++ _ = ?o2 ++ _ |- _] =>
+      eapply exec_finished_deterministic_prefix in H; [|apply H0| apply H1]
+  | [ H: Language.exec' ?u ?o1 ?s ?p (Finished _ _),
+      H0: Language.exec' ?u ?o2 ?s ?p (Crashed _),
+      H1: ?o1 ++ _ = ?o2 ++ _ |- _] =>
+      exfalso; eapply finished_not_crashed_oracle_prefix; [apply H| apply H1 | apply H0]
+  | [ H: Language.exec' ?u ?o1 ?s ?p (Finished _ _),
+      H0: Language.exec' ?u (?o1 ++ _) ?s ?p (Crashed _) |- _] =>
+      exfalso; eapply finished_not_crashed_oracle_prefix in H0; eauto;
+      try solve [rewrite <- app_assoc; eauto]
+  | [ H: Language.exec' ?u ?o1 ?s ?p (Finished _ _),
+      H0: exec _ ?u (?o1 ++ _) ?s ?p (Crashed _) |- _] =>
+      exfalso; eapply finished_not_crashed_oracle_prefix in H0; eauto;
+      try solve [rewrite <- app_assoc; eauto]
+  | [ H: Language.exec' ?u ?o1 ?s ?p (Finished _ _),
+      H0: exec _ ?u ?o2 ?s ?p (Crashed _),
+      H1: ?o1 ++ _ = ?o2 |- _] =>
+      exfalso; eapply finished_not_crashed_oracle_prefix in H0; eauto;
+      try solve [rewrite <- app_assoc; setoid_rewrite app_nil_r at 2; eauto]
+  end.
+
+  Lemma ATCD_ORS_compositional:
+  forall l_selector u T (p1 p2: prog ATCLang T) T' (p3 p4: T -> prog ATCLang T') rec P RS RSR, 
+  (forall l_selector, oracle_refines_same_from_related ATCD_Refinement u p1 p2 rec (ATCD_reboot_list l_selector) RS) ->
+  
+  (forall u o oa s1 s2 s1' s2' r1 r2 grs,
+  Language.exec' u o s1 (ATCD_Refinement.(Simulation.Definitions.compile) p1) (Finished s1' r1) ->
+  Language.exec' u o s2 (ATCD_Refinement.(Simulation.Definitions.compile) p2) (Finished s2' r2) ->
+  refines_related ATCD_Refinement RS s1 s2 ->
+  oracle_refines _ _ ATCDLang ATCLang ATCD_CoreRefinement T u s1 p1 grs o oa ->
+  oracle_refines  _ _ ATCDLang ATCLang ATCD_CoreRefinement T u s2 p2 grs o oa ->
+  oracle_refines_same_from_related ATCD_Refinement u (p3 r1) (p4 r2) rec (ATCD_reboot_list l_selector) P) ->
+  
+  (forall l_selector, oracle_refines_same_from_related_reboot _ _ _ _ ATCD_Refinement u rec rec rec (ATCD_reboot_list l_selector) RSR) ->
+  
+  (forall u o1 o2 o3 o4 oa1 oa2 s1 s2 s1' s2' r1 r2 grs,
+  Language.exec' u o1 s1 (ATCD_Refinement.(Simulation.Definitions.compile) p1) (Finished s1' r1) ->
+  Language.exec' u o2 s2 (ATCD_Refinement.(Simulation.Definitions.compile) p2) (Finished s2' r2) ->
+  oracle_refines _ _ ATCDLang ATCLang ATCD_CoreRefinement T u s1 p1 grs o1 oa1 ->
+  oracle_refines _ _ ATCDLang ATCLang ATCD_CoreRefinement T u s2 p2 grs o2 oa2 ->
+  o1 ++ o3 = o2 ++ o4 ->
+  refines_related ATCD_Refinement RS s1 s2 ->
+  o1 = o2) ->
+  
+  (forall T (p: prog ATCLang T) s s' r o o_abs grs, 
+  Language.exec' u o s (ATCD_Refinement.(Simulation.Definitions.compile) p) (Finished s' r) ->
+  oracle_refines _ _ _ _ ATCD_CoreRefinement T u s p grs o o_abs ->
+  forall grs', oracle_refines _ _ _ _ ATCD_CoreRefinement T u s p grs' o o_abs) ->
+  
+  (forall u o oa1 oa2 s1 s2 s1' s2' r1 r2 grs,
+  Language.exec' u o s1 (ATCD_Refinement.(Simulation.Definitions.compile) p1) (Finished s1' r1) ->
+  Language.exec' u o s2 (ATCD_Refinement.(Simulation.Definitions.compile) p2) (Finished s2' r2) ->
+  refines_related ATCD_Refinement RS s1 s2 ->
+  oracle_refines _ _ ATCDLang ATCLang ATCD_CoreRefinement _ u s1 p1 grs o oa1 ->
+  oracle_refines _ _ ATCDLang ATCLang ATCD_CoreRefinement _ u s2 p2 grs o oa2 ->
+  refines_related ATCD_Refinement P s1' s2') ->
+
+  (forall u o1 o2 oa1 oa2 s1 s2 s1' s2' r1,
+  Language.exec' u o1 s1 (ATCD_Refinement.(Simulation.Definitions.compile) p1) (Finished s1' r1) ->
+  refines_related ATCD_Refinement RS s1 s2 ->
+  oracle_refines _ _ ATCDLang ATCLang ATCD_CoreRefinement T u s1 p1 (ATCD_reboot_f (hd (fun _ => 0) l_selector)) o1 oa1 ->
+  oracle_refines _ _ ATCDLang ATCLang ATCD_CoreRefinement T u s2 p2 (ATCD_reboot_f (hd (fun _ => 0) l_selector)) (o1++o2) oa2 ->
+  ~Language.exec' u (o1 ++ o2) s2 (ATCD_Refinement.(Simulation.Definitions.compile) p2) (Crashed s2')) ->
+
+  (forall u o1 o2 oa1 oa2 s1 s2 s1' s2' r2,
+  Language.exec' u o1 s2 (ATCD_Refinement.(Simulation.Definitions.compile) p2) (Finished s2' r2) ->
+  refines_related ATCD_Refinement RS s1 s2 ->
+  oracle_refines _ _ ATCDLang ATCLang ATCD_CoreRefinement T u s1 p1 (ATCD_reboot_f (hd (fun _ => 0) l_selector)) (o1++o2) oa1 ->
+  oracle_refines _ _ ATCDLang ATCLang ATCD_CoreRefinement T u s2 p2 (ATCD_reboot_f (hd (fun _ => 0) l_selector)) o1 oa2 ->
+  ~Language.exec' u (o1 ++ o2) s1 (ATCD_Refinement.(Simulation.Definitions.compile) p1) (Crashed s1')) ->
+  
+  (forall u o oa1 oa2 s1 s2 s1' s2',
+  Language.exec' u o s1 (ATCD_Refinement.(Simulation.Definitions.compile) (Bind p1 p3)) (Crashed s1') ->
+  Language.exec' u o s2 (ATCD_Refinement.(Simulation.Definitions.compile) (Bind p2 p4)) (Crashed s2') ->
+  refines_related ATCD_Refinement RS s1 s2 ->
+  oracle_refines _ _ ATCDLang ATCLang ATCD_CoreRefinement _ u s1 (Bind p1 p3) (ATCD_reboot_f (hd (fun _ => 0) l_selector)) o oa1 ->
+  oracle_refines _ _ ATCDLang ATCLang ATCD_CoreRefinement _ u s2 (Bind p2 p4) (ATCD_reboot_f (hd (fun _ => 0) l_selector)) o oa2 ->
+  refines_related_reboot _ _ _ _ ATCD_Refinement RSR ((ATCD_reboot_f (hd (fun _ => 0) l_selector)) s1') ((ATCD_reboot_f (hd (fun _ => 0) l_selector)) s2')) ->
+
+  oracle_refines_same_from_related ATCD_Refinement u (Bind p1 p3) (Bind p2 p4) rec (ATCD_reboot_list l_selector) RS.
+  Proof.
+      unfold oracle_refines_same_from_related,
+      ATCD_reboot_list; 
+      simpl; intros; destruct l_selector; simpl in *; intuition.
+      {
+        destruct l_o_imp; simpl in *; try tauto;
+      cleanup; simpl in *; try congruence; try lia;
+      try solve [cleanup; tauto].
+      {  
+        repeat split_ors; cleanup;
+        try solve [cleanup; tauto].
+        repeat match goal with
+        | [H: exec ATCDLang _ _ _ (Bind _ _) _ |- _] =>
+        invert_exec'' H
+        end.
+        repeat match goal with
+        | [H: forall _, _ |- _] =>
+        specialize (H (ATCD_reboot_f (fun _ => 0)))
+        end.
+        repeat split_ors; cleanup; repeat unify_execs; cleanup.
+        match goal with
+        | [H: exec _ _ (?o ++ _) ?s ?p _,
+        H0: Language.exec' _ ?o ?s ?p _ |- _] =>
+        exfalso; eapply finished_not_crashed_oracle_prefix in H; eauto;
+        rewrite <- app_assoc; eauto
+        end.
+        match goal with
+        | [H: exec _ _ (?o1 ++ _) ?s ?p _,
+        H0: Language.exec' _ _ ?s ?p _ |- _] =>
+        exfalso; eapply finished_not_crashed_oracle_prefix in H; eauto;
+        rewrite <- app_assoc; eauto;
+        setoid_rewrite app_nil_r at 2; eauto
+        end.
+        match goal with
+        | [H: exec _ _ (?o1 ++ _) ?s ?p _,
+        H0: Language.exec' _ _ ?s ?p _ |- _] =>
+        exfalso; eapply finished_not_crashed_oracle_prefix in H; eauto;
+        rewrite <- app_assoc; eauto;
+        setoid_rewrite app_nil_r at 2; eauto
+        end.
+  
+        match goal with
+        | [H: exec _ _ _ ?s ?p (Finished _ _),
+          H0: Language.exec' _ _ ?s ?p (Finished _ _) |- _] =>
+        eapply exec_finished_deterministic_prefix in H; try solve [apply H0];
+        eauto; cleanup
+        end.
+        match goal with
+        | [H: exec _ _ _ ?s ?p (Finished _ _),
+          H0: Language.exec' _ _ ?s ?p (Finished _ _) |- _] =>
+        eapply exec_finished_deterministic_prefix in H; try solve [apply H0];
+        eauto; cleanup
+        end.
+        match goal with
+        | [H: _++_ = ?l++?l0,
+          H0: _++_ = ?l++?l0 |- _] =>
+        rewrite <- H in H0; clear_lists; subst
+        end.
+        repeat match goal with
+        | [H: exec _ _ ?o ?s ?p _,
+          H0: Language.exec' _ ?o ?s ?p _ |- _] =>
+        eapply_fresh  exec_deterministic_wrt_oracle in H; try solve [apply H0];
+        eauto; cleanup
+        end.
+  
+        match goal with
+        | [H: Language.exec' _ ?o1 ?s1 _ (Finished _ _),
+          H0: Language.exec' _ ?o2 ?s2 _ (Finished _ _),
+          H1: ?o1 ++ _ = ?o2 ++ _,
+          A2: oracle_refines _ _ _ _ _ _ _ _ _ _ ?o1 _, 
+          A3: oracle_refines _ _ _ _ _ _ _ _ _ _ ?o2 _,
+          A4: refines_related _ _ ?s1 ?s2 |- _] =>
+          specialize H2 with (1:=H)(2:= H0)(3:= A2)(4:=A3)(5:=H1)(6:= A4); subst; cleanup
+        end.
+        
+
+        specialize (H [] [x3] [x12] [x5]).
+        simpl in *.
+        specialize H with (1 := H8).
+        simpl in *.
+        assert ([x12] = [x5]). {
+          eapply H.
+        intuition; left; do 2 eexists; 
+        intuition eauto.
+        intuition; left; do 2 eexists; 
+        intuition eauto.
+        }
+        cleanup.
+        match goal with
+        | [A: Language.exec' _ _ ?s1_imp _ (Finished _ _),
+          A0: Language.exec' _ _ ?s2_imp _ (Finished _ _),
+          A1: refines_related _ _ ?s1_imp ?s2_imp,
+          A2: oracle_refines _ _ _ _ _ _ _ ?s1_imp _ _ _ _, 
+          A3: oracle_refines _ _ _ _ _ _ _ ?s2_imp _ _ _ _ |- _] =>
+          specialize H0 with (1:=A)(2:= A0)(3:= A1)(4:=A2)(5:=A3); subst; cleanup
+        end.
+        specialize (H0 [x4] [x13] [x6]).
+        eapply_fresh H4 in H19; eauto.
+
+        eapply_fresh exec_compiled_preserves_refinement_finished in H19; eauto.
+        eapply_fresh exec_compiled_preserves_refinement_finished in H20; eauto.
+        cleanup.
+        assert ([x13] = [x6]). {
+          eapply H0.
+          eauto.
+          simpl.
+          intuition; left; do 2 eexists; 
+          intuition eauto.
+          simpl.
+          intuition; left; do 2 eexists; 
+          intuition eauto.
+        }
+        cleanup; eauto.
+        unfold refines_related in *; simpl in *; cleanup; eauto.
+        unfold refines_related in *; simpl in *; cleanup; eauto.
+        match goal with
+        | [H: ?o ++ _ = _ ++ _ |- ?o ++ _ = _ ++ _] =>
+        rewrite H; eauto
+        end.
+      }
+    }
+      {
+        destruct l_o_imp; 
+        simpl in *; cleanup; try tauto.
+        repeat split_ors; cleanup; simpl in *;
+        try solve [cleanup; try tauto; try lia].
+        {  
+        repeat split_ors; cleanup;
+        try solve [cleanup; tauto].
+        repeat match goal with
+        | [H: exec ATCDLang _ _ _ (Bind _ _) _ |- _] =>
+        invert_exec'' H
+        end.
+        repeat match goal with
+        | [H: forall _, _ |- _] =>
+        specialize (H (ATCD_reboot_f t))
+        end.
+        repeat split_ors; cleanup; repeat unify_execs; cleanup.
+        match goal with
+        | [H: exec _ _ (?o ++ _) ?s ?p _,
+        H0: Language.exec' _ ?o ?s ?p _ |- _] =>
+        exfalso; eapply finished_not_crashed_oracle_prefix in H; eauto;
+        rewrite <- app_assoc; eauto
+        end.
+        match goal with
+        | [H: exec _ _ (?o1 ++ _) ?s ?p _,
+        H0: Language.exec' _ _ ?s ?p _ |- _] =>
+        exfalso; eapply finished_not_crashed_oracle_prefix in H; eauto;
+        rewrite <- app_assoc; eauto;
+        setoid_rewrite app_nil_r at 2; eauto
+        end.
+        match goal with
+        | [H: exec _ _ (?o1 ++ _) ?s ?p _,
+        H0: Language.exec' _ _ ?s ?p _ |- _] =>
+        exfalso; eapply finished_not_crashed_oracle_prefix in H; eauto;
+        rewrite <- app_assoc; eauto;
+        setoid_rewrite app_nil_r at 2; eauto
+        end.
+  
+        match goal with
+        | [H: exec _ _ _ ?s ?p (Finished _ _),
+          H0: Language.exec' _ _ ?s ?p (Finished _ _) |- _] =>
+        eapply exec_finished_deterministic_prefix in H; try solve [apply H0];
+        eauto; cleanup
+        end.
+        match goal with
+        | [H: exec _ _ _ ?s ?p (Finished _ _),
+          H0: Language.exec' _ _ ?s ?p (Finished _ _) |- _] =>
+        eapply exec_finished_deterministic_prefix in H; try solve [apply H0];
+        eauto; cleanup
+        end.
+        match goal with
+        | [H: _++_ = ?l++?l0,
+          H0: _++_ = ?l++?l0 |- _] =>
+        rewrite <- H in H0; clear_lists; subst
+        end.
+        repeat match goal with
+        | [H: exec _ _ ?o ?s ?p _,
+          H0: Language.exec' _ ?o ?s ?p _ |- _] =>
+        eapply_fresh  exec_deterministic_wrt_oracle in H; try solve [apply H0];
+        eauto; cleanup
+        end.
+  
+        match goal with
+        | [H: Language.exec' _ ?o1 ?s1 _ (Finished _ _),
+          H0: Language.exec' _ ?o2 ?s2 _ (Finished _ _),
+          H1: ?o1 ++ _ = ?o2 ++ _,
+          A2: oracle_refines _ _ _ _ _ _ _ _ _ _ ?o1 _, 
+          A3: oracle_refines _ _ _ _ _ _ _ _ _ _ ?o2 _,
+          A4: refines_related _ _ ?s1 ?s2 |- _] =>
+          specialize H2 with (1:=H)(2:= H0)(3:= A2)(4:=A3)(5:=H1)(6:= A4); subst; cleanup
+        end.
+        
+        
+        specialize (H [] [x3] [x12] [x5]).
+        simpl in *.
+        specialize H with (1 := H8).
+        simpl in *.
+        assert ([x12] = [x5]). {
+          eapply H.
+        intuition; left; do 2 eexists; 
+        intuition eauto.
+        intuition; left; do 2 eexists; 
+        intuition eauto.
+        }
+        cleanup.
+        match goal with
+        | [A: Language.exec' _ _ ?s1_imp _ (Finished _ _),
+          A0: Language.exec' _ _ ?s2_imp _ (Finished _ _),
+          A1: refines_related _ _ ?s1_imp ?s2_imp,
+          A2: oracle_refines _ _ _ _ _ _ _ ?s1_imp _ _ _ _, 
+          A3: oracle_refines _ _ _ _ _ _ _ ?s2_imp _ _ _ _ |- _] =>
+          specialize H0 with (1:=A)(2:= A0)(3:= A1)(4:=A2)(5:=A3); subst; cleanup
+        end.
+        specialize (H0 [x4] [x13] [x6]).
+        eapply_fresh H4 in H18; eauto.
+        eapply_fresh exec_compiled_preserves_refinement_finished in H18; eauto.
+        eapply_fresh exec_compiled_preserves_refinement_finished in H19; eauto.
+        cleanup.
+        assert ([x13] = [x6]). {
+          eapply H0.
+          eauto.
+          simpl.
+          intuition; left; do 2 eexists; 
+          intuition eauto.
+          simpl.
+          intuition; left; do 2 eexists; 
+          intuition eauto.
+        }
+        cleanup; eauto.
+        unfold refines_related in *; simpl in *; cleanup; eauto.
+        unfold refines_related in *; simpl in *; cleanup; eauto.
+        match goal with
+        | [H: ?o ++ _ = _ ++ _ |- ?o ++ _ = _ ++ _] =>
+        rewrite H; eauto
+        end.
+      }
+      eapply_fresh H1 in H16; eauto.
+      specialize (Hx H14); subst.
+      
+      repeat match goal with
+        | [H: exec ATCDLang _ _ _ (Bind _ _) _ |- _] =>
+        invert_exec'' H
+        end.
+      {
+        repeat split_ors; cleanup; repeat unify_execs; cleanup.
+        match goal with
+        | [H: exec _ _ (?o ++ _) ?s ?p _,
+        H0: Language.exec' _ ?o ?s ?p _ |- _] =>
+        exfalso; eapply finished_not_crashed_oracle_prefix in H; eauto;
+        rewrite <- app_assoc; eauto
+        end.
+        match goal with
+        | [H: exec _ _ (?o1 ++ _) ?s ?p _,
+        H0: Language.exec' _ _ ?s ?p _ |- _] =>
+        exfalso; eapply finished_not_crashed_oracle_prefix in H; eauto;
+        rewrite <- app_assoc; eauto;
+        setoid_rewrite app_nil_r at 2; eauto
+        end.
+        match goal with
+        | [H: exec _ _ (?o1 ++ _) ?s ?p _,
+        H0: Language.exec' _ _ ?s ?p _ |- _] =>
+        exfalso; eapply finished_not_crashed_oracle_prefix in H; eauto;
+        rewrite <- app_assoc; eauto;
+        setoid_rewrite app_nil_r at 2; eauto
+        end.
+  
+        match goal with
+        | [H: exec _ _ _ ?s ?p (Finished _ _),
+          H0: Language.exec' _ _ ?s ?p (Finished _ _) |- _] =>
+        eapply exec_finished_deterministic_prefix in H; try solve [apply H0];
+        eauto; cleanup
+        end.
+        match goal with
+        | [H: exec _ _ _ ?s ?p (Finished _ _),
+          H0: Language.exec' _ _ ?s ?p (Finished _ _) |- _] =>
+        eapply exec_finished_deterministic_prefix in H; try solve [apply H0];
+        eauto; cleanup
+        end.
+        match goal with
+        | [H: _++_ = ?l++?l0,
+          H0: _++_ = ?l++?l0 |- _] =>
+        rewrite <- H in H0; clear_lists; subst
+        end.
+        repeat match goal with
+        | [H: exec _ _ ?o ?s ?p _,
+          H0: Language.exec' _ ?o ?s ?p _ |- _] =>
+        eapply_fresh  exec_deterministic_wrt_oracle in H; try solve [apply H0];
+        eauto; cleanup
+        end.
+  
+        match goal with
+        | [H: Language.exec' _ ?o1 ?s1 _ (Finished _ _),
+          H0: Language.exec' _ ?o2 ?s2 _ (Finished _ _),
+          H1: ?o1 ++ _ = ?o2 ++ _,
+          A2: oracle_refines _ _ _ _ _ _ _ _ _ _ ?o1 _, 
+          A3: oracle_refines _ _ _ _ _ _ _ _ _ _ ?o2 _,
+          A4: refines_related _ _ ?s1 ?s2 |- _] =>
+          specialize H2 with (1:=H)(2:= H0)(3:= A2)(4:=A3)(5:=H1)(6:= A4); subst; cleanup
+        end.
+        
+        specialize H4 with (1:= H22) (2:= H23) (3:= H8).
+        specialize (H l_selector [x1] [x10] [x3]).
+        simpl in *.
+        specialize H with (1 := H8).
+        simpl in *.
+        assert ([x10] = [x3]). {
+          eapply H.
+        intuition; left; do 2 eexists; 
+        intuition eauto.
+
+        intuition; left; do 2 eexists; 
+        intuition eauto.
+        }
+        cleanup_no_match.
+        match goal with
+        | [A: Language.exec' _ _ ?s1_imp _ (Finished _ _),
+          A0: Language.exec' _ _ ?s2_imp _ (Finished _ _),
+          A1: refines_related _ _ ?s1_imp ?s2_imp,
+          A2: oracle_refines _ _ _ _ _ _ _ ?s1_imp _ _ _ _, 
+          A3: oracle_refines _ _ _ _ _ _ _ ?s2_imp _ _ _ _ |- _] =>
+          specialize H0 with (1:=A)(2:= A0)(3:= A1)(4:=A2)(5:=A3); subst; cleanup_no_match
+        end.
+        specialize (H0 (x2::l_o_imp) (x11::l) (x4::l)).
+        assert ((x11::l) = (x4::l)). {
+          eapply H0.
+          eapply H4; eauto.
+          simpl; intuition eauto.
+          simpl; intuition eauto.
+        }
+        cleanup; eauto.
+        match goal with
+        | [H: ?o ++ _ = _ ++ _ |- ?o ++ _ = _ ++ _] =>
+        rewrite H; eauto
+        end.
+      }
+      {
+        repeat split_ors; cleanup; repeat unify_execs; cleanup.
+        match goal with
+        | [H: exec _ _ (?o ++ _) ?s ?p _,
+        H0: Language.exec' _ ?o ?s ?p _ |- _] =>
+        exfalso; eapply finished_not_crashed_oracle_prefix in H; eauto;
+        rewrite <- app_assoc; eauto
+        end.
+        match goal with
+        | [H: exec _ _ (?o1 ++ _) ?s ?p _,
+        H0: Language.exec' _ _ ?s ?p _ |- _] =>
+        exfalso; eapply finished_not_crashed_oracle_prefix in H; eauto;
+        rewrite <- app_assoc; eauto;
+        setoid_rewrite app_nil_r at 2; eauto
+        end.
+
+        match goal with
+        | [H: exec _ _ _ ?s ?p (Finished _ _),
+          H0: Language.exec' _ _ ?s ?p (Finished _ _) |- _] =>
+        eapply exec_finished_deterministic_prefix in H; try solve [apply H0];
+        eauto; cleanup
+        end.
+
+        exfalso; eauto.
+
+        match goal with
+        | [H: Language.exec' _ (?o1 ++ _) ?s ?p _,
+        H0: exec _ _ _ ?s ?p _ |- _] =>
+        exfalso; eapply finished_not_crashed_oracle_prefix in H; eauto;
+        rewrite <- app_assoc; eauto;
+        setoid_rewrite app_nil_r at 2; eauto
+        end.
+      }
+      {
+        repeat split_ors; cleanup; repeat unify_execs; cleanup.
+        match goal with
+        | [H: exec _ _ (?o ++ _) ?s ?p _,
+        H0: Language.exec' _ ?o ?s ?p _ |- _] =>
+        exfalso; eapply finished_not_crashed_oracle_prefix in H; eauto;
+        rewrite <- app_assoc; eauto
+        end.
+        
+
+        match goal with
+        | [H: exec _ _ _ ?s ?p (Finished _ _),
+          H0: Language.exec' _ _ ?s ?p (Finished _ _) |- _] =>
+        eapply exec_finished_deterministic_prefix in H; try solve [apply H0];
+        eauto; cleanup
+        end.
+
+        exfalso; eauto.
+
+        match goal with
+        | [H: exec _ _ (?o1 ++ _) ?s ?p _,
+        H0: Language.exec' _ _ ?s ?p _ |- _] =>
+        exfalso; eapply finished_not_crashed_oracle_prefix in H; eauto;
+        rewrite <- app_assoc; eauto;
+        setoid_rewrite app_nil_r at 2; eauto
+        end.
+
+        match goal with
+        | [H: Language.exec' _ (?o1 ++ _) ?s ?p _,
+        H0: exec _ _ _ ?s ?p _ |- _] =>
+        exfalso; eapply finished_not_crashed_oracle_prefix in H; eauto;
+        rewrite <- app_assoc; eauto;
+        setoid_rewrite app_nil_r at 2; eauto
+        end.
+      }
+      {
+        repeat split_ors; cleanup; repeat unify_execs; cleanup.
+        specialize (H (t::l_selector) (o::l_o_imp) (o1::l) (o0::l)).
+        simpl in *.
+        specialize H with (1 := H8).
+        simpl in *.
+        {
+          eapply H.
+          intuition; right; do 2 eexists; 
+          intuition eauto.
+
+          intuition; right; do 2 eexists; 
+          intuition eauto.
+        }
+        match goal with
+        | [H: Language.exec' _ (?o ++ _) ?s ?p _,
+          H0: exec _ _ ?o ?s ?p _ |- _] =>
+        exfalso; eapply finished_not_crashed_oracle_prefix in H; eauto;
+        rewrite <- app_assoc; eauto
+        end.
+        match goal with
+        | [H: Language.exec' _ (?o ++ _) ?s ?p _,
+          H0: exec _ _ ?o ?s ?p _ |- _] =>
+        exfalso; eapply finished_not_crashed_oracle_prefix in H; eauto;
+        rewrite <- app_assoc; eauto
+        end.
+        match goal with
+        | [H: Language.exec' _ (?o ++ _) ?s ?p _,
+          H0: exec _ _ ?o ?s ?p _ |- _] =>
+        exfalso; eapply finished_not_crashed_oracle_prefix in H; eauto;
+        rewrite <- app_assoc; eauto
+        end.
+      }
+      {
+        eapply H7; eauto.
+      } 
+    }
+    Unshelve.
+    all: eauto.
+  Qed.
+
+
+
+  Opaque LogCache.recover.
+  Lemma ATCD_ORS_recover:
+      forall l_selector u R,
+      oracle_refines_same_from_related_reboot _ _ _ _ ATCD_Refinement u
+      (Simulation.Definitions.compile ATC_Refinement File.recover)
+      (Simulation.Definitions.compile ATC_Refinement File.recover)
+      (Simulation.Definitions.compile ATC_Refinement File.recover)
+      (ATCD_reboot_list l_selector) R. (* (ATCLang_related_states_reboot u' ex). *)
+      Proof.
+        Transparent File.recover.
+        unfold oracle_refines_same_from_related_reboot, 
+        ATCD_reboot_list; induction l_selector; simpl in *.
+        { (* Finished *)
+          intros.
+          unfold File.recover in *; simpl in *.
+          destruct l_o_imp; simpl in *; intuition.
+          cleanup; try tauto.
+          repeat split_ors; cleanup;
+          simpl in *; try lia.
+          specialize (H7 (ATCD_reboot_f (fun _ => 0))).
+          specialize (H4 (ATCD_reboot_f (fun _ => 0))).
+          cleanup.
+          repeat invert_exec; simpl in *; cleanup.
+          eapply HC_map_ext_eq in H8.
+          eapply HC_map_ext_eq in H8.
+          subst.
+
+          repeat split_ors; cleanup;
+          repeat invert_exec; simpl in *; cleanup; eauto;
+          try congruence.
+          apply HC_map_ext_eq in H7; subst.
+          apply HC_map_ext_eq in H0; subst.
+          rewrite <- H4 in *; clear H4; simpl in *; cleanup.
+    
+          repeat apply HC_map_ext_eq in H4; subst.
+          specialize (H15 tt).
+          specialize (H18 tt).
+          specialize (H26 tt).
+          specialize (H29 tt).
+          repeat split_ors; cleanup;
+          repeat invert_exec; simpl in *; cleanup; eauto;
+          try congruence.
+
+          apply HC_map_ext_eq in H11; subst.
+          apply HC_map_ext_eq in H14; subst.
+          specialize (H12 []).
+          specialize (H15 []).
+          repeat split_ors; cleanup;
+          repeat invert_exec; simpl in *; cleanup; eauto;
+          try congruence; repeat unify_execs; cleanup.
+        }
+        {(*Crashed*)
+          intros.
+          unfold TCD_reboot_list, File.recover in *; simpl in *.
+          destruct l_o_imp; simpl in *; intuition.
+          cleanup; try tauto.
+          repeat split_ors; cleanup;
+          simpl in *; try lia.
+          {
+            specialize (H7 (ATCD_reboot_f a)).
+            specialize (H4 (ATCD_reboot_f a)).
+            cleanup.
+            repeat invert_exec; simpl in *; cleanup.
+            eapply HC_map_ext_eq in H8.
+            eapply HC_map_ext_eq in H8.
+            subst.
+
+            repeat split_ors; cleanup;
+            repeat invert_exec; simpl in *; cleanup; eauto;
+            try congruence.
+            apply HC_map_ext_eq in H7; subst.
+          apply HC_map_ext_eq in H0; subst.
+          rewrite <- H4 in *; clear H4; simpl in *; cleanup.
+    
+          repeat apply HC_map_ext_eq in H4; subst.
+            specialize (H15 tt).
+            specialize (H18 tt).
+            specialize (H26 tt).
+            specialize (H29 tt).
+            repeat split_ors; cleanup;
+            repeat invert_exec; simpl in *; cleanup; eauto;
+            try congruence.
+
+            apply HC_map_ext_eq in H11; subst.
+            apply HC_map_ext_eq in H14; subst.
+            specialize (H12 []).
+            specialize (H15 []).
+            repeat split_ors; cleanup;
+            repeat invert_exec; simpl in *; cleanup; eauto;
+            try congruence; repeat unify_execs; cleanup.
+          }
+          {
+            cleanup.
+            repeat invert_exec; simpl in *; cleanup.
+            repeat split_ors; cleanup; try congruence;
+            repeat invert_exec; simpl in *; cleanup; eauto;
+            try congruence.
+            {
+              specialize (H11 tt).
+              specialize (H15 tt).
+              cleanup.
+              eapply IHl_selector in H5.
+              3: apply H7.
+              2:{
+                unfold refines_related_reboot in *;
+                cleanup.
+                eexists (_, (_, _)), (_, (_, _)); split; eauto.
+                2: split; eauto.
+                {
+                  simpl in *; unfold HC_refines_reboot in *;
+                  simpl in *; cleanup; eauto.
+                  simpl in *; unfold HC_refines_reboot in *;
+                  simpl in *; cleanup; eauto.
+                  intuition.
+                  eapply refines_reboot_to_refines_reboot; eauto.
+                }
+                {
+                  simpl in *; unfold HC_refines_reboot in *;
+                  simpl in *; cleanup; eauto.
+                  simpl in *; unfold HC_refines_reboot in *;
+                  simpl in *; cleanup; eauto.
+                  intuition.
+                  eapply refines_reboot_to_refines_reboot; eauto.
+                }
+                shelve.
+              }
+              subst; eauto.
+              simpl in *; cleanup; eauto.
+            }
+            {
+
+            cleanup.
+            repeat invert_exec; simpl in *; cleanup.
+            simpl in *; cleanup.
+            rewrite <- H2, <- H6 in *; clear H2 H6.
+          subst.
+
+          repeat split_ors; cleanup;
+          repeat invert_exec; simpl in *; cleanup; eauto;
+          try congruence.
+            }
+            {
+              cleanup.
+            repeat invert_exec; simpl in *; cleanup.
+            simpl in *; cleanup.
+            rewrite <- H8 in *; clear H8.
+            simpl in *; cleanup.
+            }
+            {
+              cleanup.
+              repeat invert_exec; simpl in *; cleanup.
+              simpl in *; cleanup.
+              rewrite  <- H6 in *; clear H6.
+              simpl in *; cleanup.
+            }
+            {
+              cleanup.
+            repeat invert_exec; simpl in *; cleanup.
+            simpl in *; cleanup.
+          repeat split_ors; cleanup;
+          repeat invert_exec; simpl in *; cleanup; eauto;
+          try congruence.
+            
+          apply HC_map_ext_eq in H8; subst.
+          rewrite <- H3 in *; clear H3; 
+          simpl in *; cleanup.
+    
+          repeat apply HC_map_ext_eq in H4; subst.
+          repeat apply HC_map_ext_eq in H8; subst.
+          repeat apply HC_map_ext_eq in H2; subst.
+          specialize (H15 tt).
+          specialize (H18 tt).
+          specialize (H28 tt).
+          specialize (H31 tt).
+          repeat split_ors; cleanup;
+          repeat invert_exec; simpl in *; cleanup; eauto;
+          try congruence.
+
+          apply HC_map_ext_eq in H8; subst.
+          apply HC_map_ext_eq in H15; subst.
+          specialize (H9 []).
+          specialize (H16 []).
+          repeat split_ors; cleanup;
+          repeat invert_exec; simpl in *; cleanup; eauto;
+          try congruence; repeat unify_execs; cleanup.
+          
+          eapply IHl_selector in H5.
+          3: apply H7.
+          2:{
+            unfold refines_related_reboot in *;
+            cleanup.
+            eexists (_, (_, _)), (_, (_, _)); split; eauto.
+            2: split; eauto.
+            {
+              simpl in *; unfold HC_refines_reboot in *;
+              simpl in *; cleanup; eauto.
+              simpl in *; unfold HC_refines_reboot in *;
+              simpl in *; cleanup; eauto.
+              intuition.
+              unfold refines_reboot in *; cleanup.
+              apply H9 in H12.
+              split.
+              repeat split_ors.
+              eapply RepImplications.cached_log_reboot_rep_to_reboot_rep; eauto.
+              eapply RepImplications.cached_log_crash_rep_during_recovery_to_reboot_rep; eauto.
+              eapply RepImplications.cached_log_crash_rep_after_commit_to_reboot_rep; eauto.
+              simpl; apply select_total_mem_synced.
+            }
+            {
+              simpl in *; unfold HC_refines_reboot in *;
+              simpl in *; cleanup; eauto.
+              simpl in *; unfold HC_refines_reboot in *;
+              simpl in *; cleanup; eauto.
+              intuition.
+              unfold refines_reboot in *; cleanup.
+              apply H6 in H4.
+              split.
+              repeat split_ors.
+              eapply RepImplications.cached_log_reboot_rep_to_reboot_rep; eauto.
+              eapply RepImplications.cached_log_crash_rep_during_recovery_to_reboot_rep; eauto.
+              eapply RepImplications.cached_log_crash_rep_after_commit_to_reboot_rep; eauto.
+              simpl; apply select_total_mem_synced.
+            }
+            shelve.
+          }
+          subst; eauto.
+        }
+      }
+    }
+    Unshelve.
+    all: try solve [exact (fun _ _ => True)].
+    all: simpl; eauto.
+Qed.
+
+
+Lemma oracle_refines_independent_from_reboot_function:
+      forall u (T : Type) (p : prog ATCLang T)
+    s s' r o o_abs grs,
+    Language.exec' u o s (Simulation.Definitions.compile ATCD_Refinement p)
+    (Finished s' r) ->
+    oracle_refines _ _ ATCDLang ATCLang
+    ATCD_CoreRefinement T u s p grs o o_abs ->
+    forall grs',
+    oracle_refines _ _ ATCDLang ATCLang
+    ATCD_CoreRefinement T u s p grs' o o_abs.
+    Proof.
+      induction p; simpl; eauto.
+      intros. 
+      {
+        destruct o; simpl in *; cleanup.
+        {
+          invert_exec'' H; repeat invert_exec;
+          eexists; intuition eauto.
+        }
+        {
+          eapply lift2_invert_exec in H; cleanup.
+          apply HC_map_ext_eq in H; eauto; subst.
+          specialize (H3 tt); simpl in *.
+          destruct o; simpl in *.
+          {
+            cleanup; invert_exec'' H1; 
+            repeat invert_exec;
+            eexists; intuition eauto;
+            do 2 eexists; intuition eauto;
+            simpl; intuition eauto. 
+            all: simpl; eauto.
+          }
+          {
+            eapply lift2_invert_exec in H1; cleanup.
+          apply HC_map_ext_eq in H; eauto; subst.
+          specialize (H5 []); simpl in *.
+          destruct o; simpl in *.
+          {
+            split_ors; cleanup; repeat unify_execs; cleanup.
+            eexists; intuition eauto;
+            do 2 eexists; intuition eauto;
+            simpl; intuition eauto.
+            do 2 eexists; intuition eauto.
+          }
+          {
+            repeat split_ors; cleanup; repeat unify_execs; cleanup.
+            eexists; intuition eauto;
+            do 2 eexists; intuition eauto;
+            simpl; intuition eauto.
+            do 2 eexists; intuition eauto.
+
+            repeat split_ors; cleanup; repeat unify_execs; cleanup.
+          }
+          {
+            repeat split_ors; cleanup; repeat unify_execs; cleanup.
+            eexists; intuition eauto;
+            do 2 eexists; intuition eauto;
+            simpl; intuition eauto.
+            do 2 eexists; intuition eauto.
+          } 
+          {
+            repeat split_ors; cleanup; repeat unify_execs; cleanup.
+            eexists; intuition eauto;
+            do 2 eexists; intuition eauto;
+            simpl; intuition eauto.
+            do 2 eexists; intuition eauto.
+          }
+        }
+      }
+    }
+    {
+      intros.
+      invert_exec'' H0.
+      split_ors; cleanup.
+      match goal with
+      | [H: exec _ _ (?o ++ _) ?s ?p _,
+        H0: Language.exec' _ ?o ?s ?p _ |- _] =>
+        exfalso; eapply finished_not_crashed_oracle_prefix in H; eauto;
+        rewrite <- app_assoc; eauto
+      end.
+      match goal with
+      | [H: exec _ _ _ ?s ?p (Finished _ _),
+        H0: Language.exec' _ _ ?s ?p (Finished _ _) |- _] =>
+      eapply exec_finished_deterministic_prefix in H; try solve [apply H0];
+      eauto; cleanup
+      end.
+      repeat match goal with
+      | [H: exec _ _ ?o ?s ?p _,
+        H0: Language.exec' _ ?o ?s ?p _ |- _] =>
+      eapply_fresh  exec_deterministic_wrt_oracle in H; try solve [apply H0];
+      eauto; cleanup
+      end.
+    
+      right.
+      do 7 eexists; intuition eauto.
+      Unshelve.
+      all: eauto.
+    }
+Qed.
+(*
+    Lemma HC_oracle_refines_lift2:
+    forall T (p: TD.(prog) T) o u s x,
+    oracle_refines _ _ATCDLang ATCLang
+    (HC_Core_Refinement ATCDLang ATCLang Definitions.TDCoreRefinement)
+    T u s
+    (lift_L2 AuthenticationOperation p)
+    (fun
+    s : HorizontalComposition.state' AuthenticationOperation
+          TransactionCacheOperation => (fst s, ([], snd (snd s))))
+    o
+    (map
+    (fun
+        o : Language.token'
+              (TransactionalDiskLayer.TDCore data_length) =>
+      match o with
+      | OpToken _ o1 =>
+          OpToken
+            (HorizontalComposition AuthenticationOperation
+              (TransactionalDiskLayer.TDCore data_length))
+            (Token2 AuthenticationOperation
+              (TransactionalDiskLayer.TDCore data_length) o1)
+      | Language.Crash _ =>
+          Language.Crash
+            (HorizontalComposition AuthenticationOperation
+              (TransactionalDiskLayer.TDCore data_length))
+      | Language.Cont _ =>
+          Language.Cont
+            (HorizontalComposition AuthenticationOperation
+              (TransactionalDiskLayer.TDCore data_length))
+      end) x) ->
+    
+      ((RefinementLift.compile
+    (HorizontalComposition AuthenticationOperation
+        TransactionCacheOperation)
+    (HorizontalComposition AuthenticationOperation
+        (TransactionalDiskLayer.TDCore data_length)) ATCDLang ATCLang
+    (HC_Core_Refinement ATCDLang ATCLang Definitions.TDCoreRefinement) T
+    (lift_L2 AuthenticationOperation p)) = 
+    (lift_L2 AuthenticationOperation 
+    (RefinementLift.compile TransactionCacheOperation
+    (TransactionalDiskLayer.TDCore data_length) Definitions.imp TD
+    Definitions.TDCoreRefinement T p))) ->
+    
+      exists o',
+      oracle_refines _ _ Definitions.imp TD Definitions.TDCoreRefinement
+      T u (snd s) p (fun s => ([], snd s)) o' x /\
+      HC_oracle_transformation o o'.
+      Proof.
+        induction p; simpl; intuition eauto.
+        {
+          cleanup.
+          specialize (H3 tt).
+          eexists; intuition eauto.
+          eexists; intuition eauto.
+          destruct x; simpl in *; cleanup; try congruence.
+          destruct x; simpl in *; cleanup; try congruence; eauto.
+        }
+        {
+          cleanup.
+        destruct x; simpl in *; cleanup; try congruence; eauto.
+        destruct x; simpl in *; cleanup; try congruence; eauto.
+        eexists; intuition eauto.
+        left; eexists; intuition eauto.
+        econstructor.
+        invert_exec.
+        eexists; intuition eauto.
+        simpl; eauto.
+        }
+        {
+          cleanup.
+            destruct x; simpl in *; cleanup; try congruence; eauto.
+            destruct x; simpl in *; cleanup; try congruence; eauto.
+            eexists; intuition eauto.
+            right; do 2 eexists; intuition eauto.
+            econstructor.
+            invert_exec.
+            eexists; intuition eauto.
+            simpl; eauto.
+          }
+          {
+            cleanup.
+            inversion H1; cleanup; eauto.
+            edestruct IHp; eauto; cleanup.
+            simpl in *.
+            eexists; intuition eauto.
+            eapply lift2_invert_exec_crashed in H0; cleanup.
+            apply HC_map_ext_eq in H6; subst.
+            left; eexists; intuition eauto.
+          }
+          {
+            cleanup.
+            inversion H1; cleanup; eauto.
+            destruct (Compare_dec.le_dec (length x2) (length x)). 
+            {
+              rewrite <- firstn_skipn with (l:= x)(n:= length x2) in H2.
+              rewrite map_app in H2.
+              apply app_split_length_eq_l in H2; eauto; cleanup.
+              eapply FunctionalExtensionality.equal_f with (x3:= x5) in H8; eauto.
+            
+              rewrite <- H0 in *.
+              edestruct IHp; eauto; cleanup.
+              edestruct H; eauto; cleanup.
+    
+              eapply lift2_invert_exec in H3; cleanup.
+              apply HC_map_ext_eq in H2; subst.
+              destruct x6.
+              {
+                eapply lift2_invert_exec in H4; cleanup.
+                apply HC_map_ext_eq in H10; subst.
+                eexists; intuition eauto.
+                right; do 7 eexists; intuition eauto.
+                rewrite firstn_skipn; eauto.
+                apply HC_oracle_transformation_merge;
+                eapply HC_oracle_transformation_same.
+              }
+              {
+                eapply lift2_invert_exec_crashed in H4; cleanup.
+                apply HC_map_ext_eq in H10; subst.
+                eexists; intuition eauto.
+                right; do 7 eexists; intuition eauto.
+                rewrite firstn_skipn; eauto.
+                apply HC_oracle_transformation_merge;
+                eapply HC_oracle_transformation_same.
+              }
+              rewrite map_length, firstn_length_l; eauto.
+            }
+            {
+              eapply f_equal in H2.
+              rewrite map_length, app_length in H2; try lia.
+            }
+          }
+      Qed.
+*)
+    
+
+Definition LD_have_same_structure {T T'} (p1: LoggedDiskLayer.logged_disk_prog T) 
+(p2: LoggedDiskLayer.logged_disk_prog T') :=
+  match p1, p2 with
+  | LoggedDiskLayer.Read _, LoggedDiskLayer.Read _ => True
+  | LoggedDiskLayer.Write _ _, LoggedDiskLayer.Write _ _ => True
+  | LoggedDiskLayer.Recover, LoggedDiskLayer.Recover => True
+  | LoggedDiskLayer.Init _, LoggedDiskLayer.Init _ => True
+  | _, _ => False
+  end.
+
+Definition TC_have_same_structure {T T'} (p1: TransactionCacheLayer.TransactionCacheOperation.(operation) T) 
+  (p2: TransactionCacheLayer.TransactionCacheOperation.(operation) T') :=
+    match p1, p2 with
+    | P1 p1 , P1 p2 =>
+      match p1, p2 with  
+      | ListLayer.Get _, ListLayer.Get _ => True
+      | ListLayer.Put _, ListLayer.Put _ => True
+      | ListLayer.Delete _, ListLayer.Delete _ => True
+      | _, _ => False
+      end
+    | P2 p1, P2 p2 =>
+      LD_have_same_structure p1 p2
+    | _, _ => False
+    end.
+
+Fixpoint ATC_have_same_structure {T T'} (p1: ATCLang.(prog) T) (p2: ATCLang.(prog) T') u s1 s2 :=
+  match p1, p2 with
+  | Op _ o1, Op _ o2 =>
+    match o1, o2 with
+    | P1 _, P1 _ => True (*It can only be auth*)
+    | P2 t1, P2 t2 =>
+      TC_have_same_structure t1 t2
+    | _, _ => False
+    end
+  | Ret _, Ret _ => True
+  | @Bind _ T1_1 T1_2 p1_1 p1_2, @Bind _ T2_1 T2_2 p2_1 p2_2 =>
+    T1_1 = T2_1 /\
+    T1_2 = T2_2 /\
+    ATC_have_same_structure p1_1 p2_1 u s1 s2 /\
+    (forall o s1' r1 s2' r2,
+    exec ATCLang u o s1 p1_1 (Finished s1' r1) ->
+    exec ATCLang u o s2 p2_1 (Finished s2' r2) ->
+    ATC_have_same_structure (p1_2 r1) (p2_2 r2) u s1' s2')
+  | _, _ => False
+  end.
+
+Lemma LD_oracle_refines_operation_eq:
+forall (u0 : user) (T : Type) (o1 : operation (LoggedDiskOperation log_length data_length) T)
+(T' : Type) (o2 : operation (LoggedDiskOperation log_length data_length) T')
+x16 x17 x18 x19 x20 x21 x22 x23 s0 s3 s1' s2'
+(r1 : T) (r2 : T'),
+token_refines T u0 s0 o1 x22 x21
+x17 ->
+token_refines T' u0 s3 o2 x19 x18
+x23 ->
+exec (CachedDiskLang) u0 x21 s0
+(LoggedDiskCoreRefinement.(Simulation.Definitions.compile_core) o1) 
+(Finished s1' r1) ->
+exec (CachedDiskLang) u0 x18 s3
+(LoggedDiskCoreRefinement.(Simulation.Definitions.compile_core) o2)
+(Finished s2' r2) ->
+LD_have_same_structure o1 o2 -> 
+x18 ++ x16 = x21 ++ x20 -> x18 = x21 /\ x17 = x23.
+Proof.
+intros;
+destruct o1, o2; simpl in *; cleanup; try tauto.
+{
+  repeat split_ors; cleanup; repeat unify_execs_prefix; cleanup;
+  repeat unify_execs; cleanup.
+  eapply read_finished_oracle_eq in H1; eauto.
+}
+{
+  repeat (split_ors; cleanup; repeat unify_execs;
+  repeat unify_execs_prefix; cleanup);
+  try solve [eapply write_finished_oracle_eq in H1; eauto; cleanup; eauto].
+}
+{
+  repeat (split_ors; cleanup; repeat unify_execs;
+  repeat unify_execs_prefix; cleanup).
+  eapply recover_finished_oracle_eq in H1; eauto.
+}
+{
+  repeat (split_ors; cleanup; repeat unify_execs;
+  repeat unify_execs_prefix; cleanup).
+  eapply init_finished_oracle_eq in H1; eauto.
+  admit.
+}
+Unshelve.
+all: eauto.
+Admitted.
+
+Lemma TC_oracle_refines_operation_eq:
+forall (u0 : user) (T : Type) (o1 : operation TransactionCacheOperation T)
+(T' : Type) (o2 : operation TransactionCacheOperation T')
+x16 x17 x18 x19 x20 x21 x22 x23 s0 s3 s1' s2'
+(r1 : T) (r2 : T'),
+TCD_CoreRefinement.(Simulation.Definitions.token_refines) u0 s0 o1 x22 x21
+x17 ->
+TCD_CoreRefinement.(Simulation.Definitions.token_refines) u0 s3 o2 x19 x18
+x23 ->
+exec (TCDLang) u0 x21 s0
+(TCD_CoreRefinement.(Simulation.Definitions.compile_core) o1) 
+(Finished s1' r1) ->
+exec (TCDLang) u0 x18 s3
+(TCD_CoreRefinement.(Simulation.Definitions.compile_core) o2)
+(Finished s2' r2) ->
+TC_have_same_structure o1 o2 -> 
+x18 ++ x16 = x21 ++ x20 -> x18 = x21 /\ x17 = x23.
+Proof.
+intros;
+destruct o1, o2; simpl in *; cleanup; try tauto;
+repeat invert_exec; cleanup; eauto.
+eapply HC_map_ext_eq in H;
+eapply HC_map_ext_eq in H1; cleanup.
+apply HC_map_ext_eq_prefix in H4; eauto; cleanup.
+eapply LD_oracle_refines_operation_eq in H; eauto.
+cleanup; eauto.
+Unshelve.
+all: exact [].
+Qed.
+
+
+Lemma LD_oracle_refines_operation_eq_crashed:
+forall (u0 : user) (T : Type) (o1 : operation (LoggedDiskOperation log_length data_length) T)
+(T' : Type) (o2 : operation (LoggedDiskOperation log_length data_length) T')
+x16 x17 x18 x19 x20 x21 x22 x23 s0 s3 s1' s2',
+token_refines T u0 s0 o1 x22 x21
+x17 ->
+token_refines T' u0 s3 o2 x19 x18
+x23 ->
+exec (CachedDiskLang) u0 x21 s0
+(LoggedDiskCoreRefinement.(Simulation.Definitions.compile_core) o1) 
+(Crashed s1') ->
+exec (CachedDiskLang) u0 x18 s3
+(LoggedDiskCoreRefinement.(Simulation.Definitions.compile_core) o2)
+(Crashed s2') ->
+LD_have_same_structure o1 o2 -> 
+x18 ++ x16 = x21 ++ x20 -> x17 = x23.
+Proof.
+intros;
+destruct o1, o2; simpl in *; cleanup; try tauto.
+{
+  repeat split_ors; cleanup; repeat unify_execs_prefix; cleanup;
+  repeat unify_execs; cleanup; eauto.
+}
+{
+  repeat (split_ors; cleanup; repeat unify_execs;
+  repeat unify_execs_prefix; cleanup; eauto);
+  try solve [eapply write_finished_oracle_eq in H1; eauto; cleanup; eauto].
+  (* Use oracle length thing *)
+  all: admit.
+}
+{
+  repeat (split_ors; cleanup; repeat unify_execs;
+  repeat unify_execs_prefix; cleanup; eauto).
+}
+{
+  repeat (split_ors; cleanup; repeat unify_execs;
+  repeat unify_execs_prefix; cleanup; eauto).
+}
+Unshelve.
+all: eauto.
+Admitted.
+
+Lemma TC_oracle_refines_operation_eq_crashed:
+forall (u0 : user) (T : Type) (o1 : operation TransactionCacheOperation T)
+(T' : Type) (o2 : operation TransactionCacheOperation T')
+x16 x17 x18 x19 x20 x21 x22 x23 s0 s3 s1' s2',
+TCD_CoreRefinement.(Simulation.Definitions.token_refines) u0 s0 o1 x22 x21
+x17 ->
+TCD_CoreRefinement.(Simulation.Definitions.token_refines) u0 s3 o2 x19 x18
+x23 ->
+exec (TCDLang) u0 x21 s0
+(TCD_CoreRefinement.(Simulation.Definitions.compile_core) o1) 
+(Crashed s1') ->
+exec (TCDLang) u0 x18 s3
+(TCD_CoreRefinement.(Simulation.Definitions.compile_core) o2)
+(Crashed s2') ->
+TC_have_same_structure o1 o2 -> 
+x18 ++ x16 = x21 ++ x20 -> x17 = x23.
+Proof.
+intros;
+destruct o1, o2; simpl in *; cleanup; try tauto;
+repeat invert_exec; cleanup; eauto.
+eapply HC_map_ext_eq in H;
+eapply HC_map_ext_eq in H1; cleanup.
+apply HC_map_ext_eq_prefix in H4; eauto; cleanup.
+eapply LD_oracle_refines_operation_eq_crashed in H; eauto.
+cleanup; eauto.
+Unshelve.
+all: exact [].
+Qed.
+
+Lemma ATCD_oracle_refines_impl_eq:
+forall u T p1 T' p2 s1 s2 s1' s2' s1a s2a r1 r2 o1 o2 o3 o4 oa1 oa2 selector, (* oa3 oa4, *)
+oracle_refines _ _ ATCDLang ATCLang ATCD_CoreRefinement
+  T u s1 p1 (ATCD_reboot_f selector) o1 oa1 ->
+oracle_refines _ _ ATCDLang ATCLang ATCD_CoreRefinement
+  T' u s2 p2 (ATCD_reboot_f selector) o2 oa2 ->
+
+@HC_refines _ _ _ _ _ ATCLang TCD_CoreRefinement s1 s1a ->
+@HC_refines _ _ _ _ _ ATCLang TCD_CoreRefinement s2 s2a ->
+
+  exec ATCDLang u o1 s1 (ATCD_Refinement.(Simulation.Definitions.compile) p1) (Finished s1' r1) ->
+  exec ATCDLang u o2 s2 (ATCD_Refinement.(Simulation.Definitions.compile) p2) (Finished s2' r2) ->
+  ATC_have_same_structure p1 p2 u s1a s2a ->
+
+  (forall u T (o1: operation TransactionCacheOperation T) T' (o2 : operation TransactionCacheOperation T') x x0 x1 x2 x3 x4 x5 x6 s1 s2 s1' s2' r1 r2,
+  TCD_CoreRefinement.(Simulation.Definitions.token_refines) u s1 o1 x5 x4 x0 ->
+  TCD_CoreRefinement.(Simulation.Definitions.token_refines) u s2 o2 x2 x1 x6 ->
+  exec TCDLang u x4 s1
+  (TCD_CoreRefinement.(Simulation.Definitions.compile_core) o1)
+  (Finished s1' r1) ->
+  exec TCDLang u x1 s2
+  (TCD_CoreRefinement.(Simulation.Definitions.compile_core) o2)
+  (Finished s2' r2) ->
+  TC_have_same_structure o1 o2 ->
+  x1 ++ x = x4 ++ x3 ->
+  x1 = x4 /\ x0 = x6) ->
+
+o1 ++ o3 = o2 ++ o4 ->
+not_init p1 /\ not_init p2 ->
+o1 = o2 /\ oa1 = oa2.
+Proof.
+  induction p1; destruct p2; simpl; intros; try tauto; 
+  cleanup_no_match; try tauto.
+  {
+    clear H8 H9.
+    cleanup; try tauto;
+    unfold HC_token_refines in *; cleanup;
+    simpl in *; cleanup; eauto.
+
+    specialize (H9 tt).
+    specialize (H11 tt).
+    eapply_fresh HC_map_ext_eq_prefix in H7; eauto; cleanup_no_match.
+    eapply lift2_invert_exec in H3; cleanup.
+    eapply lift2_invert_exec in H4; cleanup.
+    eapply_fresh HC_map_ext_eq in H4; eauto; subst.
+    eapply_fresh HC_map_ext_eq in H0; eauto; subst.
+
+    assert (x6 = x5 /\ x3 = x1). {
+      eapply H6; eauto.
+    }
+    cleanup; eauto.
+  }
+  {
+    repeat invert_exec; eauto.
+    repeat split_ors; cleanup; 
+    simpl in *; cleanup; 
+    try congruence; eauto.
+    repeat invert_exec.
+    repeat invert_exec.
+  }
+  {
+    repeat invert_exec.
+    repeat rewrite <- app_assoc in *.
+    repeat split_ors; cleanup; repeat unify_execs_prefix;
+    cleanup; repeat unify_execs; cleanup.
+    exfalso; eapply finished_not_crashed_oracle_prefix; 
+    [eauto | | eauto];
+    rewrite <- app_assoc; eauto.
+
+    exfalso; eapply finished_not_crashed_oracle_prefix; 
+    [eauto | | eauto];
+    rewrite <- app_assoc; eauto.
+
+    exfalso; eapply finished_not_crashed_oracle_prefix in H0; eauto;
+    rewrite <- app_assoc; eauto.
+
+    eapply exec_finished_deterministic_prefix in H17; eauto; cleanup.
+    eapply exec_finished_deterministic_prefix in H22; eauto; cleanup.
+    repeat unify_execs; cleanup.
+    repeat rewrite <- app_assoc in *.
+    eapply_fresh IHp1 in H5; eauto; subst; cleanup.
+
+
+    eapply ATCD_exec_lift_finished in H4; eauto;
+    try solve [apply TransactionToTransactionalDisk.Refinement.TC_to_TD_core_simulation_finished];
+    try solve [apply TransactionToTransactionalDisk.Refinement.TC_to_TD_core_simulation_crashed];
+    try solve [apply not_init_read].
+    eapply ATCD_exec_lift_finished in H5; eauto;
+    try solve [apply TransactionToTransactionalDisk.Refinement.TC_to_TD_core_simulation_finished];
+    try solve [apply TransactionToTransactionalDisk.Refinement.TC_to_TD_core_simulation_crashed];
+    try solve [apply not_init_read].
+    simpl in *; cleanup.
+
+    eapply H in H6; eauto.
+    cleanup; eauto.
+  }
+Unshelve.
+all: eauto.
+Qed.
+
+Lemma ATCD_oracle_refines_prefix_one_crashed:
+forall u T (p1 : ATCLang.(prog) T) T' (p2 : ATCLang.(prog) T') o1 o2 o3 o4 s1 s2 s1' s2' r1 s1a s2a oa1 oa2 selector,
+oracle_refines _ _ ATCDLang ATCLang ATCD_CoreRefinement
+  T u s1 p1 (ATCD_reboot_f selector) o1 oa1 ->
+oracle_refines _ _ ATCDLang ATCLang ATCD_CoreRefinement
+  T' u s2 p2 (ATCD_reboot_f selector) o2 oa2 ->
+
+
+exec ATCDLang u o1 s1 (ATCD_Refinement.(Simulation.Definitions.compile) p1) (Finished s1' r1) ->
+exec ATCDLang u o2 s2 (ATCD_Refinement.(Simulation.Definitions.compile) p2) (Crashed s2') ->
+
+
+@HC_refines _ _ _ _ _ ATCLang TCD_CoreRefinement s1 s1a ->
+@HC_refines _ _ _ _ _ ATCLang TCD_CoreRefinement s2 s2a ->
+
+ATC_have_same_structure p1 p2 u s1a s2a ->
+not_init p1 ->
+not_init p2 ->
+o1 ++ o3 = o2 ++ o4 ->
+False.
+Proof.
+  induction p1; simpl; intros. 
+  {
+    repeat (simpl in *; cleanup; try tauto; eauto);
+    repeat invert_exec; simpl in *; cleanup; try congruence.
+    
+    (*
+    eapply lift2_invert_exec in H1; cleanup.
+    eapply lift2_invert_exec_crashed in H2; cleanup.
+    *)
+    rewrite <- H, <- H0 in *; clear H H0; 
+    simpl in *; cleanup.
+    rewrite <- H, <- H0 in *; clear H H0; 
+    simpl in *; cleanup.
+    rewrite <- H, <- H0 in *; clear H H0; 
+    simpl in *; cleanup.
+
+    repeat eapply HC_map_ext_eq in H2.
+    repeat eapply HC_map_ext_eq in H.
+    subst.
+    specialize (H11 tt).
+    specialize (H13 tt).
+    cleanup; try congruence.
+    repeat eapply HC_map_ext_eq in H2.
+    repeat eapply HC_map_ext_eq in H13.
+    subst.
+
+    eapply HC_map_ext_eq_prefix in H8; cleanup.
+    eapply HC_map_ext_eq_prefix in H; cleanup.
+    specialize (H11 []).
+    specialize (H14 []).
+    destruct o, o5; cleanup; simpl in *; 
+    try tauto; 
+    repeat split_ors; cleanup; 
+    repeat unify_execs; cleanup; 
+    try congruence.
+
+    eapply read_finished_not_crashed; eauto.
+    eapply write_finished_not_crashed; eauto.
+    eapply write_finished_not_crashed; eauto.
+    eapply recover_finished_not_crashed; eauto.
+    eapply H6; eauto.
+  }
+  {
+    repeat (simpl in *; cleanup; try tauto; eauto).
+    repeat split_ors; cleanup; eauto;
+    simpl in *; cleanup; eauto;
+    repeat invert_exec; simpl in *; cleanup.
+  }
+  {
+    repeat (simpl in *; cleanup; try tauto; eauto).
+    repeat invert_exec.
+    repeat rewrite <- app_assoc in *.
+    repeat split_ors; cleanup; eauto;
+    repeat rewrite <- app_assoc in *; eauto;
+
+    try solve [exfalso; eapply finished_not_crashed_oracle_prefix; 
+    [eauto | | eauto];
+    rewrite <- app_assoc; eauto].
+    {
+
+    eapply exec_finished_deterministic_prefix in H16; eauto; cleanup.
+    repeat unify_execs; cleanup.
+    repeat rewrite <- app_assoc in *.
+    eapply IHp1; eauto.
+    }
+    {
+      exfalso; eapply finished_not_crashed_oracle_prefix in H3; eauto. 
+      rewrite <- app_assoc; eauto.
+    }
+    {
+      exfalso; eapply finished_not_crashed_oracle_prefix in H0; eauto. 
+      rewrite <- app_assoc; eauto.
+    }
+    {
+      eapply exec_finished_deterministic_prefix in H17; eauto; cleanup.
+      eapply exec_finished_deterministic_prefix in H22; eauto; cleanup.
+      repeat unify_execs; cleanup.
+
+      eapply_fresh ATCD_oracle_refines_impl_eq in H19. 
+      7: eauto.
+      all: eauto.
+      2: apply TC_oracle_refines_operation_eq.
+      cleanup.
+      
+      eapply_fresh exec_compiled_preserves_refinement_finished in H2; eauto; 
+      cleanup; simpl in *.
+      eapply_fresh exec_compiled_preserves_refinement_finished in H14; eauto; 
+      cleanup; simpl in *.
+      eapply_fresh ATCD_exec_lift_finished in H2; eauto;
+      try solve [apply TransactionToTransactionalDisk.Refinement.TC_to_TD_core_simulation_finished];
+      try solve [apply TransactionToTransactionalDisk.Refinement.TC_to_TD_core_simulation_crashed].
+      eapply_fresh ATCD_exec_lift_finished in H14; eauto;
+      try solve [apply TransactionToTransactionalDisk.Refinement.TC_to_TD_core_simulation_finished];
+      try solve [apply TransactionToTransactionalDisk.Refinement.TC_to_TD_core_simulation_crashed].
+      simpl in *; cleanup.
+
+      eapply H.
+      7: eauto.
+      all: eauto.
+    }
+  }
+  Unshelve.
+  all: eauto.
+Qed.
+
+
+Lemma ATCD_ORS_equiv_impl:
+forall u T (p1 p2: ATCLang.(prog) T) rec l_grs (EQ1 EQ2: state ATCLang -> state ATCLang -> Prop),
+oracle_refines_same_from_related ATCD_Refinement u
+p1 p2 rec l_grs EQ2 ->
+(forall s1 s2, EQ1 s1 s2 -> EQ2 s1 s2) ->
+oracle_refines_same_from_related ATCD_Refinement u
+p1 p2 rec l_grs EQ1.
+Proof.
+  unfold oracle_refines_same_from_related; intros.
+  eapply H; eauto.
+  unfold refines_related in *; cleanup; eauto.
+  do 2 eexists; intuition eauto.
+Qed.
+
+
+Set Nested Proofs Allowed.
+Lemma ATC_have_same_structure_sym:
+forall T1 (p1 : ATCLang.(prog) T1) 
+T2 (p2 : ATCLang.(prog) T2) u s1 s2,
+ATC_have_same_structure p1 p2 u s1 s2 ->
+ATC_have_same_structure p2 p1 u s2 s1.
+Proof.
+induction p1; destruct p2; 
+simpl; intros; 
+simpl in *; cleanup; eauto.
+
+destruct o1, o2;
+simpl in *; cleanup; eauto.
+
+destruct o, o0;
+simpl in *; cleanup; eauto.
+
+intuition eauto.
+Qed.
+
+
+Lemma ATCD_oracle_refines_impl_eq_crashed:
+forall u T p1 T' p2 s1 s2 s1' s2' s1a s2a o1 o2 o3 o4 oa1 oa2 selector, (* oa3 oa4, *)
+oracle_refines _ _ ATCDLang ATCLang ATCD_CoreRefinement
+  T u s1 p1 (ATCD_reboot_f selector) o1 oa1 ->
+oracle_refines _ _ ATCDLang ATCLang ATCD_CoreRefinement
+  T' u s2 p2 (ATCD_reboot_f selector) o2 oa2 ->
+
+@HC_refines _ _ _ _ _ ATCLang TCD_CoreRefinement s1 s1a ->
+@HC_refines _ _ _ _ _ ATCLang TCD_CoreRefinement s2 s2a ->
+
+  exec ATCDLang u o1 s1 (ATCD_Refinement.(Simulation.Definitions.compile) p1) (Crashed s1') ->
+  exec ATCDLang u o2 s2 (ATCD_Refinement.(Simulation.Definitions.compile) p2) (Crashed s2') ->
+  ATC_have_same_structure p1 p2 u s1a s2a ->
+
+  (forall u T (o1: operation TransactionCacheOperation T) T' (o2 : operation TransactionCacheOperation T') x x0 x1 x2 x3 x4 x5 x6 s1 s2 s1' s2' r1 r2,
+  TCD_CoreRefinement.(Simulation.Definitions.token_refines) u s1 o1 x5 x4 x0 ->
+  TCD_CoreRefinement.(Simulation.Definitions.token_refines) u s2 o2 x2 x1 x6 ->
+  exec TCDLang u x4 s1
+  (TCD_CoreRefinement.(Simulation.Definitions.compile_core) o1)
+  (Finished s1' r1) ->
+  exec TCDLang u x1 s2
+  (TCD_CoreRefinement.(Simulation.Definitions.compile_core) o2)
+  (Finished s2' r2) ->
+  TC_have_same_structure o1 o2 ->
+  x1 ++ x = x4 ++ x3 ->
+  x1 = x4 /\ x0 = x6) ->
+
+  (forall u T (o1: operation TransactionCacheOperation T) T' (o2 : operation TransactionCacheOperation T') 
+  x x0 x1 x2 x3 x4 x5 x6 s1 s2 s1' s2',
+  TCD_CoreRefinement.(Simulation.Definitions.token_refines) u s1 o1 x5 x4 x0 ->
+  TCD_CoreRefinement.(Simulation.Definitions.token_refines) u s2 o2 x2 x1 x6 ->
+  exec TCDLang u x4 s1
+  (TCD_CoreRefinement.(Simulation.Definitions.compile_core) o1)
+  (Crashed s1') ->
+  exec TCDLang u x1 s2
+  (TCD_CoreRefinement.(Simulation.Definitions.compile_core) o2)
+  (Crashed s2') ->
+  TC_have_same_structure o1 o2 ->
+  x1 ++ x = x4 ++ x3 ->
+  x0 = x6) ->
+
+o1 ++ o3 = o2 ++ o4 ->
+not_init p1 /\ not_init p2 ->
+oa1 = oa2.
+Proof.
+  induction p1; destruct p2; simpl; intros; try tauto; 
+  cleanup_no_match; try tauto.
+  {
+    clear H9 H10.
+    cleanup; try tauto;
+    unfold HC_token_refines in *; cleanup;
+    simpl in *; cleanup; eauto.
+
+    specialize (H10 tt).
+    specialize (H12 tt).
+    eapply_fresh HC_map_ext_eq_prefix in H8; eauto; cleanup_no_match.
+    eapply lift2_invert_exec_crashed in H3; cleanup.
+    eapply lift2_invert_exec_crashed in H4; cleanup.
+    eapply_fresh HC_map_ext_eq in H4; eauto; subst.
+    eapply_fresh HC_map_ext_eq in H0; eauto; subst.
+
+    assert (x3 = x1). {
+      eapply H7; eauto.
+    }
+    cleanup; eauto.
+  }
+  {
+    repeat invert_exec; eauto.
+    repeat split_ors; cleanup; 
+    simpl in *; cleanup; 
+    try congruence; eauto.
+    repeat invert_exec.
+    repeat invert_exec.
+  }
+  {
+    repeat invert_exec.
+    repeat rewrite <- app_assoc in *.
+    repeat split_ors; cleanup; repeat unify_execs_prefix;
+    cleanup; repeat unify_execs; cleanup.
+    eapply IHp1; eauto.
+
+
+    exfalso; eapply finished_not_crashed_oracle_prefix in H17.
+    eapply H17; eauto.
+    rewrite <- app_assoc; eauto.
+
+    exfalso; eapply finished_not_crashed_oracle_prefix in H14.
+    eapply H14; eauto.
+    rewrite <- app_assoc; eauto.
+
+
+    exfalso; eapply finished_not_crashed_oracle_prefix in H21.
+    eapply H21; eauto.
+    rewrite <- app_assoc; eauto.
+
+    exfalso; eapply finished_not_crashed_oracle_prefix in H0; eauto.
+    rewrite <- app_assoc; eauto.
+
+    rewrite <- app_assoc in *.
+    eapply exec_finished_deterministic_prefix in H19; eauto; cleanup.
+    exfalso; eapply ATCD_oracle_refines_prefix_one_crashed.
+    4: eauto.
+    6: eauto.
+    8: eauto.
+    all: eauto.
+
+    exfalso; eapply finished_not_crashed_oracle_prefix in H0; eauto.
+    rewrite <- app_assoc; eauto.
+
+    exfalso; eapply finished_not_crashed_oracle_prefix in H5; eauto.
+    rewrite <- app_assoc; eauto.
+
+    exfalso; eapply finished_not_crashed_oracle_prefix in H1; eauto.
+    rewrite <- app_assoc; eauto.
+
+    rewrite <- app_assoc in *.
+    eapply exec_finished_deterministic_prefix in H18; eauto; cleanup.
+    exfalso; eapply ATCD_oracle_refines_prefix_one_crashed.
+    4: apply H4.
+    3: apply H6.
+    5: eapply ATC_have_same_structure_sym; eauto.
+    all: eauto.
+
+
+    exfalso; eapply finished_not_crashed_oracle_prefix in H4; eauto;
+    rewrite <- app_assoc; eauto.
+
+    exfalso; eapply finished_not_crashed_oracle_prefix in H1; eauto;
+    rewrite <- app_assoc; eauto.
+
+    exfalso; eapply finished_not_crashed_oracle_prefix in H0; eauto;
+    rewrite <- app_assoc; eauto.
+
+    eapply exec_finished_deterministic_prefix in H20; eauto; cleanup.
+    eapply exec_finished_deterministic_prefix in H25; eauto; cleanup.
+    repeat unify_execs; cleanup.
+    repeat rewrite <- app_assoc in *.
+    eapply_fresh ATCD_oracle_refines_impl_eq in H6.
+    7: eauto.
+    all: eauto.
+    cleanup.
+
+    eapply ATCD_exec_lift_finished in H6; eauto;
+    try solve [apply TransactionToTransactionalDisk.Refinement.TC_to_TD_core_simulation_finished];
+    try solve [apply TransactionToTransactionalDisk.Refinement.TC_to_TD_core_simulation_crashed];
+    try solve [apply not_init_read].
+    eapply ATCD_exec_lift_finished in H17; eauto;
+    try solve [apply TransactionToTransactionalDisk.Refinement.TC_to_TD_core_simulation_finished];
+    try solve [apply TransactionToTransactionalDisk.Refinement.TC_to_TD_core_simulation_crashed];
+    try solve [apply not_init_read].
+    simpl in *; cleanup.
+
+    eapply H in H14.
+    6: eauto.
+    2: eauto.
+    2: eauto.
+    all: eauto.
+    cleanup; eauto.
+  }
+Unshelve.
+all: eauto.
+Qed.
+
+
+
+Lemma ATCD_ORS_transfer:
+forall (l_selector: list (@total_mem addr addr_dec nat)) 
+T (p1 p2: AD.(prog) T)  u u' ex,
+
+ATCSimulation.not_init p1 ->
+ATCSimulation.not_init p2 ->
+
+(forall s1 s2, 
+(refines_related ATC_Refinement (AD_related_states u' ex)) s1 s2 ->
+ATC_have_same_structure (Simulation.Definitions.compile ATC_Refinement p1)
+(Simulation.Definitions.compile ATC_Refinement p2) u s1 s2) ->
+
+oracle_refines_same_from_related ATCD_Refinement u
+(Simulation.Definitions.compile ATC_Refinement p1)
+(Simulation.Definitions.compile ATC_Refinement p2)
+(Simulation.Definitions.compile ATC_Refinement File.recover)
+(ATCD_reboot_list l_selector) 
+(refines_related ATC_Refinement (AD_related_states u' ex)).
+Proof.
+  unfold ATCD_reboot_list, TCD_reboot_list; induction l_selector; intros.
+  {
+    unfold oracle_refines_same_from_related; intros.
+    simpl in *.
+    destruct l_o_imp; simpl in *; try tauto.
+    cleanup; try tauto.
+    simpl in *; repeat split_ors; cleanup; try tauto.
+    unfold refines_related at 1 in H2; cleanup; eauto.
+    simpl in *. 
+    eapply ATCD_oracle_refines_impl_eq in H10.
+    5: apply H5.
+    all: eauto.
+    3: apply TC_oracle_refines_operation_eq.
+    cleanup; eauto.
+    all: shelve.
+  }
+  {
+    unfold oracle_refines_same_from_related; intros.
+    simpl in *.
+    destruct l_o_imp; simpl in *; try tauto.
+    cleanup; try tauto.
+    unfold refines_related at 1 in H2; cleanup; eauto.
+    simpl in *; repeat split_ors; cleanup; try tauto.
+    {
+      simpl in *. 
+      eapply ATCD_oracle_refines_impl_eq in H12.
+      5: apply H5.
+      all: eauto.
+      3: apply TC_oracle_refines_operation_eq.
+      cleanup; eauto.
+      all: shelve.
+    }
+    {
+      simpl in *.
+      exfalso; eapply ATCD_oracle_refines_prefix_one_crashed.
+      3: eauto.
+      3: eauto.
+      all: eauto.
+      all: shelve.
+    }
+    {
+      simpl in *.
+      exfalso; eapply ATCD_oracle_refines_prefix_one_crashed.
+      3: eauto.
+      3: eauto.
+      all: eauto.
+      all: shelve.
+    }
+    {
+      simpl in *. 
+      eapply_fresh ATCD_oracle_refines_impl_eq_crashed in H11.
+      5: apply H5.
+      all: eauto.
+      3: apply TC_oracle_refines_operation_eq.
+      3: apply TC_oracle_refines_operation_eq_crashed.
+      cleanup; eauto.
+      eapply ATCD_ORS_recover in H10.
+      apply H10 in H12; 
+      subst; eauto.
+      all: shelve.
+    }
+  }
+  Unshelve.
+  all: eauto.
+  all: try split.
+  all: try solve [eapply not_init_compile; eauto].
+  all: try solve [ 
+    apply H1 in H8; eauto; apply ATC_have_same_structure_sym; eauto].
+  exact (fun _ => 0).
+  exact (fun _ _ => True).
+  {
+    unfold refines_related_reboot in *; cleanup; simpl in *.
+    eapply ATCD_exec_lift_crashed in H6; eauto;
+  try solve [apply TransactionToTransactionalDisk.Refinement.TC_to_TD_core_simulation_finished];
+  try solve [apply TransactionToTransactionalDisk.Refinement.TC_to_TD_core_simulation_crashed].
+  eapply ATCD_exec_lift_crashed in H7; eauto;
+  try solve [apply TransactionToTransactionalDisk.Refinement.TC_to_TD_core_simulation_finished];
+  try solve [apply TransactionToTransactionalDisk.Refinement.TC_to_TD_core_simulation_crashed].
+  cleanup.
+
+
+  unfold ATCD_refines_reboot in *; simpl in *.
+  unfold HC_refines_reboot; simpl;
+  unfold HC_refines_reboot; simpl.
+  eexists (_, (_, _)), (_, (_, _)).
+  simpl; intuition eauto.
+  all: eapply not_init_compile; eauto.
+  }
+Qed.
